src/Implementations/BlockAllocator/BlockAllocator.v
@@ -1,2 +1,141 @@
-Require Export BlockAllocator.Definitions.
-Require Export BlockAllocator.Facts.
+Require Import Framework FSParameters TransactionalDiskLayer Omega.
+Import IfNotations.
+Close Scope pred_scope.
+
+Notation "| p |" := (Op (TransactionalDiskOperation data_length) p)(at level 60).
+Notation "x <-| p1 ; p2" := (Bind (Op (TransactionalDiskOperation data_length) p1) (fun x => p2))(right associativity, at level 60). 
+
+Definition valid_bitlist l := length l = block_size /\ (forall i, In i l -> i < 2).
+
+Record bitlist :=
+  {
+   bits : list nat;                
+   valid : valid_bitlist bits
+  }.
+
+Fixpoint get_first_zero l :=
+  match l with
+  | nil => 0
+  | hd::tl =>
+    match hd with
+    | O => 0
+    | _ => S (get_first_zero tl)
+    end
+  end.
+
+Theorem upd_valid_zero:
+  forall i l,
+    valid_bitlist l ->
+    valid_bitlist (updN l i 0).
+Proof.
+  unfold valid_bitlist in *; intros; cleanup.
+  rewrite length_updN; intuition.
+  apply in_updN in H1; intuition; eauto.
+Qed.
+
+Theorem upd_valid_one:
+  forall i l,
+    valid_bitlist l ->
+    valid_bitlist (updN l i 1).
+Proof.
+  unfold valid_bitlist in *; intros; cleanup.
+  rewrite length_updN; intuition.
+  apply in_updN in H1; intuition; eauto.
+Qed.
+
+Axiom value_to_bits: value -> bitlist.
+Axiom bits_to_value: bitlist -> value.
+Axiom value_to_bits_to_value : forall v, bits_to_value (value_to_bits v) = v.
+Axiom bits_to_value_to_bits : forall l, value_to_bits (bits_to_value l) = l.   
+
+Module Type BlockAllocatorParameters.
+  Parameter bitmap_addr: addr.
+  Parameter num_of_blocks: nat.
+  Parameter num_of_blocks_in_bounds: num_of_blocks <= block_size.
+End BlockAllocatorParameters.
+  
+(* This is a generic block allocator which has a 1 block bitmap and num_of_blocks blocks following it *)  
+Module BlockAllocator (Params : BlockAllocatorParameters).
+
+Import Params.
+  
+Definition alloc (v': value) :=
+  v <-| Read bitmap_addr;
+  let bits := bits (value_to_bits v) in
+  let valid := valid (value_to_bits v) in
+  let index := get_first_zero (firstn num_of_blocks bits) in
+  
+  if lt_dec index num_of_blocks then
+    _ <-| Write (S index) v';
+    _ <-| Write bitmap_addr
+      (bits_to_value (Build_bitlist (updN bits index 1)
+                     (upd_valid_one index bits valid)));
+    Ret (Some index)
+  else
+    Ret None.
+
+Definition free a :=
+  if lt_dec a num_of_blocks then
+  v <-| Read bitmap_addr;
+  let bits := bits (value_to_bits v) in
+  let valid := valid (value_to_bits v) in
+  if nth_error bits a is Some 1 then
+      _ <-| Write bitmap_addr (bits_to_value (Build_bitlist (updN bits a 0) (upd_valid_zero a bits valid)));
+      Ret (Some tt)
+    else
+      Ret None
+  else
+    Ret None.
+
+Definition read a :=
+  if lt_dec a num_of_blocks then
+  v <-| Read bitmap_addr;
+  let bits := bits (value_to_bits v) in
+  let valid := valid (value_to_bits v) in
+  if nth_error bits a is Some 1 then
+      v <-| Read (S a);
+      Ret (Some v)
+    else
+      Ret None
+  else
+    Ret None.
+
+Definition write a b :=
+  if lt_dec a num_of_blocks then
+  v <-| Read bitmap_addr;
+  let bits := bits (value_to_bits v) in
+  let valid := valid (value_to_bits v) in
+  if nth_error bits a is Some 1 then
+      _ <-| Write (S a) b;
+      Ret (Some tt)
+    else
+      Ret None
+  else
+    Ret None.
+
+Open Scope pred_scope.
+  
+Fixpoint ptsto_bits' (dh: disk value) value_sets bits n : @pred addr addr_dec (set value) :=
+  match value_sets, bits with
+  | vs::value_sets', b::bits' =>
+    (S n) |-> vs *
+    match b with
+    | 0 => [[ dh n = None ]]
+    | 1 => [[ dh n = Some (fst vs) ]]
+    | _ => [[ False ]]
+    end *
+    ptsto_bits' dh value_sets' bits' (S n)
+   | _, _ =>
+    emp
+  end.
+      
+Definition ptsto_bits dh value_sets bits := ptsto_bits' dh value_sets bits 0.
+
+Definition block_allocator_rep (dh: disk value) : @pred addr addr_dec (set value) :=
+  (exists* bitmap bl value_sets,
+     let bits := bits (value_to_bits bitmap) in
+     bitmap_addr |-> (bitmap, bl) *
+     ptsto_bits dh value_sets bits *
+     [[ length value_sets = num_of_blocks ]] *
+     [[ forall i, i >= num_of_blocks -> dh i = None ]])%pred.
+End BlockAllocator.
