src/Implementations/File/File.v
@@ -1,1 +1,143 @@
-Require Export Implementations.File.Definitions.
+Require Import Framework FSParameters AuthenticatedDiskLayer BlockAllocator Inode.
+Import IfNotations.
+
+Open Scope pred_scope.
+
+Module DiskAllocatorParams <: BlockAllocatorParameters.
+  Definition bitmap_addr := file_blocks_start.
+  Definition num_of_blocks := file_blocks_count.
+  Definition num_of_blocks_in_bounds := file_blocks_count_in_bounds.
+End DiskAllocatorParams.
+
+Module DiskAllocator := BlockAllocator DiskAllocatorParams.
+
+Record File :=
+  {
+    owner: user;
+    blocks: list value;
+  }.
+
+Definition file_rep (file: File) (inode: Inode) (file_block_map: disk value) :=
+  file.(owner) = inode.(Inode.owner) /\
+  length file.(blocks) = length inode.(block_numbers) /\
+  (forall i block_number,
+       nth_error inode.(block_numbers) i = Some block_number ->
+       nth_error file.(blocks) i = file_block_map block_number).
+
+Definition files_inner_rep file_map inode_map file_block_map :=
+   addrs_match file_map inode_map /\
+   (forall inum inode file,
+     inode_map inum  = Some inode ->
+     file_map inum = Some file ->
+     file_rep file inode file_block_map).
+
+Definition files_rep (file_map: disk File) :=
+  exists* inode_map file_block_map,
+    inode_rep inode_map *
+    DiskAllocator.block_allocator_rep file_block_map *
+    [[ files_inner_rep file_map inode_map file_block_map ]].
+
+Local Definition auth_then_exec {T} (inum: Inum) (p: Inum -> prog (TransactionalDiskLang data_length) (option T)) :=
+  _ <- |ADDO| Start;
+  mo <- |ADDP| get_owner inum;
+  if mo is Some owner then
+    ok <- |ADAO| Auth owner;
+    if ok is Some tt then
+      r <- |ADDP| p inum;
+      if r is Some v then
+        _ <- |ADDO| Commit;
+        Ret (Some v)
+      else
+        _ <- |ADDO| Abort;
+        Ret None
+    else
+      _ <- |ADDO| Abort;
+      Ret None
+  else
+    _ <- |ADDO| Abort;
+    Ret None.
+        
+Local Definition read_inner off inum :=
+  r <- get_block_number inum off;
+  if r is Some block_number then
+    r <- DiskAllocator.read block_number;
+    if r is Some v then
+      Ret (Some v)
+    else
+      Ret None
+  else
+    Ret None.
+
+Local Definition write_inner off v inum :=
+  r <- get_block_number inum off;
+  if r is Some block_number then
+    r <- DiskAllocator.write block_number v;
+    if r is Some tt then
+      Ret (Some tt)
+    else
+      Ret None
+  else
+    Ret None.
+
+Local Definition change_owner_inner owner inum :=
+  r <- change_owner inum owner;
+  if r is Some tt then
+     Ret (Some tt)
+  else
+    Ret None.
+
+Local Fixpoint free_all_blocks block_nums :=
+  match block_nums with
+  | nil =>
+    Ret (Some tt)
+  | bn :: block_nums' =>
+    ok <- DiskAllocator.free bn;
+    if ok is Some tt then
+      r <- free_all_blocks block_nums';
+      Ret r
+    else
+      Ret None
+end.
+
+Local Definition delete_inner inum :=
+  mbl <- get_block_numbers inum;
+  if mbl is Some block_numbers then
+    ok <- free_all_blocks block_numbers;
+    if ok is Some tt then
+      r <- free inum;
+      if r is Some tt then
+        Ret (Some tt)
+      else
+        Ret None
+    else
+      Ret None
+  else
+    Ret None.
+
+Local Definition extend_inner v inum :=
+  mbn <- DiskAllocator.alloc v;
+  if mbn is Some block_num then
+    r <- extend inum block_num;
+    if r is Some tt then
+      Ret (Some tt)
+    else
+      Ret None
+  else
+    Ret None.
+
+
+Definition read inum off := auth_then_exec inum (read_inner off).
+Definition write inum off v := auth_then_exec inum (write_inner off v).
+Definition extend inum v := auth_then_exec inum (extend_inner v).
+Definition change_owner inum owner := auth_then_exec inum (change_owner_inner owner).
+Definition delete inum := auth_then_exec inum delete_inner.
+
+Definition create owner :=
+  _ <- |ADDO| Start;
+  r <- |ADDP| alloc owner;
+  if r is Some inum then
+     _ <- |ADDO| Commit;
+     Ret (Some inum)
+  else
+    _ <- |ADDO| Abort;
+    Ret None.
