src/Extraction/Extraction.v
@@ -1,0 +1,51 @@
+From Coq Require Extraction.
+Require Import ExtrHaskellBasic.
+Require Import ExtrHaskellNatInteger.
+Require Import ExtrHaskellZInteger.
+Require Import ExtrHaskellString.
+Extraction Language Haskell.
+
+Require Import Framework FSParameters.
+Require LogCache Transaction File.
+
+Extract Inlined Constant addr => "Prelude.Integer".
+Extract Constant user => "Prelude.Int".
+Extract Constant value => "Prelude.Int".
+Extract Constant file_blocks_count => "4096".
+Extract Constant log_length => "500".
+Extract Constant inode_count => "4096".
+Extract Constant disk_size => "10 Prelude.* 4096".
+
+(* Eliminate Horizontal Composition *) 
+Extraction Implicit lift_L1 [ 1 2 ].
+Extraction Implicit lift_L2 [ 1 2 ]. 
+Extract Inlined Constant lift_L1 => "".
+Extract Inlined Constant lift_L2 => "".
+
+Extraction Inline Operation.prog.
+Extraction Inline Language.prog. 
+
+Extract Inductive Language.prog' => "Prelude.IO" [ "" "Prelude.return" "(Prelude.>>=)" ].
+
+(* Use these to implement actual functionality
+Extract Inductive DiskLayer.disk_prog => "Prelude.IO" [ "DISK_READ" "DISK_WRITE"  ].
+Extract Inductive CryptoLayer.crypto_prog => "Prelude.IO" [ "GET_KEY" "HASH" "ENCRYPT" "DECRYPT" ].
+Extract Inductive CacheLayer.cache_prog => "Prelude.IO" [ "CACHE_READ" "CACHE_WRITE" "CACHE_FLUSH"]. 
+Extract Inductive AuthenticationLayer.authentication_prog => "Prelude.IO" [ "AUTHENTICATE" ].
+Extract Inductive StorageLayer.storage_prog => "Prelude.IO" [ "GET" "PUT" "DELETE" ].
+*)
+
+Extract Inductive LoggedDiskLayer.logged_disk_prog => "Prelude.IO" [ "LogCache.read" "LogCache.write" ].
+Extract Inductive TransactionalDiskLayer.transactional_disk_prog => "Prelude.IO" [ "Transaction.start" "Transaction.read" "Transaction.write" "Transaction.commit" "Transaction.abort" ].
+
+Separate Extraction
+           File.read File.write
+           File.change_owner File.extend
+           File.delete File.create
+           Transaction.start Transaction.read
+           Transaction.write Transaction.commit
+           Transaction.abort
+           LogCache.read LogCache.write.
+
+
+
