src/Framework/Simulation/RefinementLift.v
@@ -1,0 +1,50 @@
+Require Import Primitives Layer Simulation.Definitions.
+
+Section RefinementLift.
+  Variable O1 O2: Operation.
+  Variable L1: Language O1.
+  Variable L2: Language O2.
+  Variable OpRefinement : OperationRefinement L1 O2.
+
+  Fixpoint compile T (p2: prog L2 T) : prog L1 T.
+    destruct p2.
+    exact (OpRefinement.(compile_op) p).
+    exact (Ret t).
+    exact (Bind (compile T p2) (fun x => compile T' (p x))).
+  Defined.
+
+  Fixpoint oracle_refines_to T (d1: state L1) (p: prog L2 T) o1 o2 : Prop :=
+    match p with    
+    |Op _ op =>
+     exists o2',
+     o2 =  [OpOracle O2 o2' ] /\
+     OpRefinement.(oracle_refines_to_op) d1 op o1 o2'
+
+    | Ret v =>
+      (exists d1',
+         exec L1 o1 d1 (Ret v) (Crashed d1') /\
+         o2 = [Crash _]) \/
+      (exists d1' r,
+         exec L1 o1 d1 (Ret v) (Finished d1' r) /\
+         o2 = [Cont _])
+
+    | @Bind _ T1 T2 p1 p2 =>
+      exists o1' o1'' o2' o2'',
+      o1 = o1'++o1'' /\
+      o2 = o2' ++ o2'' /\
+     ((exists d1', exec L1 o1' d1 (compile T1 p1) (Crashed d1') /\
+         oracle_refines_to T1 d1 p1 o1' o2') \/
+      (exists d1' r ret,
+         exec L1 o1' d1 (compile T1 p1) (Finished d1' r) /\
+         exec L1 o1'' d1' (compile T2 (p2 r)) ret /\
+         oracle_refines_to T1 d1 p1 o1' o2' /\
+         oracle_refines_to T2 d1' (p2 r) o1'' o2''
+         ))
+    end.
+
+  Definition LiftRefinement : Refinement L1 L2 := Build_Refinement compile OpRefinement.(refines_to_op) oracle_refines_to.
+
+End RefinementLift.
+
+Arguments LiftRefinement {_ _ _}.
+
