src/Implementations/BatchOperations/BatchOperations.v
@@ -1,1 +1,55 @@
-Require Export BatchOperations.Definitions BatchOperations.Specs.
+Require Import Framework CryptoDiskLayer.
+
+  Fixpoint write_consecutive a vl :=
+  match vl with
+  | nil => Ret tt
+  | v::vl' =>
+    _ <- |DO| Write a v;
+    _ <- write_consecutive (S a) vl';
+    Ret tt
+  end.
+
+  Fixpoint read_consecutive a count:=
+    match count with
+    | 0 => Ret nil
+    | S count' =>
+      v <- |DO| Read _ a;
+      vl <- read_consecutive (S a) count';
+    Ret (v::vl)
+  end.
+
+Fixpoint write_batch al vl :=
+  match al, vl with
+  | a::al', v::vl' =>
+    _ <- |DO| Write a v;
+    _ <- write_batch al' vl';
+    Ret tt            
+  | _, _ => Ret tt
+  end.
+  
+Fixpoint encrypt_all k vl :=
+  match vl with
+  | nil => Ret nil
+  | v::vl' =>
+    ev <- |CO| Encrypt k v;
+    evl' <- encrypt_all k vl';
+    Ret (ev::evl')
+  end.
+
+Fixpoint decrypt_all k evl :=
+  match evl with
+  | nil => Ret nil
+  | ev::evl' =>
+    v <- |CO| Decrypt k ev;
+    vl' <- decrypt_all k evl';
+    Ret (v::vl')
+  end.
+
+Fixpoint hash_all h vl :=
+  match vl with
+  | nil => Ret h
+  | v::vl' =>
+    h' <- |CO| Hash h v;
+    h'' <- hash_all h' vl';
+    Ret h''
+  end.
