src/Implementations/Inode/Inode.v
@@ -1,1 +1,96 @@
-Require Export Inode.Definitions.
+Require Import Transaction. (* Needed for extraction *)
+Require Import Framework FSParameters TransactionalDiskLayer BlockAllocator.
+Import IfNotations.
+
+Definition Inum := addr.
+
+Record Inode :=
+  {
+    owner: user;
+    block_numbers : list addr;
+  }.
+
+Variable encode_inode : Inode -> value.
+Variable decode_inode: value -> Inode.
+Axiom inode_encode_decode:
+  forall i,
+    decode_inode (encode_inode i) = i.
+Axiom inode_decode_encode:
+  forall b,
+    encode_inode (decode_inode b) = b.
+
+Module InodeAllocatorParams <: BlockAllocatorParameters.
+  Definition bitmap_addr := inode_blocks_start.
+  Definition num_of_blocks := inode_count.
+  Definition num_of_blocks_in_bounds := inode_count_in_bounds.
+End InodeAllocatorParams.
+
+Module InodeAllocator := BlockAllocator InodeAllocatorParams.
+
+Import InodeAllocator.
+
+Open Scope pred_scope.
+
+Definition inode_map_rep inode_block_map (inode_map: disk Inode) :=
+  forall i, inode_map i = option_map decode_inode (inode_block_map i).
+
+Definition inode_rep (inode_map: disk Inode) : @pred addr addr_dec (set value) :=
+  exists* inode_block_map,
+    block_allocator_rep inode_block_map *
+    [[ forall i, inode_map i = option_map decode_inode (inode_block_map i) ]].
+
+Local Definition get_inode inum :=
+  r <- read inum;
+  if r is Some i then
+    Ret (Some (decode_inode i))
+  else
+    Ret None.
+
+Local Definition set_inode inum inode:=
+  r <- write inum (encode_inode inode);
+  Ret r.
+
+Definition alloc user :=
+  r <- alloc (encode_inode (Build_Inode user []));
+  Ret r.
+
+Definition free inum :=
+  r <- free inum;
+  Ret r.
+
+Definition extend inum block_num :=
+  r <- get_inode inum;
+  if r is Some inode then
+    r <- set_inode inum (Build_Inode inode.(owner) (inode.(block_numbers)++[block_num]));
+      Ret r
+  else
+    Ret None.
+
+Definition change_owner inum user :=
+  r <- get_inode inum;
+  if r is Some inode then
+    r <- set_inode inum (Build_Inode user inode.(block_numbers));
+      Ret r
+  else
+    Ret None.
+
+Definition get_block_number inum off:=
+  r <- get_inode inum;
+  if r is Some inode then
+    Ret (nth_error inode.(block_numbers) off)
+  else
+    Ret None.
+
+Definition get_block_numbers inum :=
+  r <- get_inode inum;
+  if r is Some inode then
+    Ret (Some inode.(block_numbers))
+  else
+    Ret None.
+
+Definition get_owner inum :=
+  r <- get_inode inum;
+  if r is Some inode then
+    Ret (Some inode.(owner))
+  else
+    Ret None.
