src/Layers/AbstractLayers/FileDisk/FileDiskLayer.v
@@ -1,0 +1,1047 @@
+Require Import Omega Framework File.
+Import ListNotations.
+Close Scope pred_scope.
+
+Set Implicit Arguments.
+
+Section FileDisk.
+
+  Variable disk_size : nat.
+  Notation "'Inum'" := addr.
+
+  Inductive token' :=
+  | CrashBefore : token'
+  | CrashAfter : token'
+  | CrashAfterCreate : Inum -> token'
+  | NewInum : Inum -> token'
+  | InodesFull : token'
+  | DiskFull : token'
+  | Cont : token'.
+
+  Definition token_dec' : forall (t t': token'), {t=t'}+{t<>t'}.
+    decide equality.
+    all: apply  addr_dec.
+  Defined.
+
+  Definition oracle' := list token'.  
+
+  Definition state' := (user * disk File)%type.
+  
+  Inductive file_disk_prog : Type -> Type :=
+  | Read : Inum -> addr -> file_disk_prog (option value)
+  | Write : Inum -> addr -> value -> file_disk_prog (option unit)
+  | Extend : Inum -> value -> file_disk_prog (option unit)
+  | SetOwner : Inum -> user -> file_disk_prog (option unit)
+  | Create : user -> file_disk_prog (option addr)
+  | Delete : Inum -> file_disk_prog (option unit).
+  
+  Inductive exec' :
+    forall T, oracle' ->  state' -> file_disk_prog T -> @Result state' T -> Prop :=
+  | ExecReadSuccess : 
+      forall s inum off file v,
+        let u := fst s in
+        let d := snd s in
+        inum < disk_size ->
+        d inum = Some file ->
+        file.(owner) = u ->
+        nth_error file.(blocks) off = Some v ->
+        exec' [Cont] s (Read inum off) (Finished s (Some v))
+              
+  | ExecReadFail : 
+      forall s inum off file,
+        let u := fst s in
+        let d := snd s in
+        (inum >= disk_size \/
+         d inum = None \/
+         d inum = Some file /\
+         (file.(owner) <> u \/ nth_error file.(blocks) off = None)) ->
+        exec' [Cont] s (Read inum off) (Finished s None)
+              
+  | ExecWriteSuccess :
+      forall s inum file off v,
+        let u := fst s in
+        let d := snd s in
+        inum < disk_size ->
+        d inum = Some file ->
+        file.(owner) = u ->
+        off < length (file.(blocks)) ->
+        let new_file := Build_File file.(owner) (firstn off file.(blocks) ++ v :: skipn (S off) file.(blocks)) in
+        exec' [Cont] s (Write inum off v) (Finished (u, (upd d inum new_file)) (Some tt))
+
+  | ExecWriteFail :
+      forall s inum file off v,
+        let u := fst s in
+        let d := snd s in
+        (inum >= disk_size \/
+         d inum = None \/
+         d inum = Some file /\
+         (file.(owner) <> u \/ off >= length (file.(blocks)))) ->
+        exec' [Cont] s (Write inum off v) (Finished s None)
+
+  | ExecExtendSuccess :
+      forall s inum file v,
+        let u := fst s in
+        let d := snd s in
+        inum < disk_size ->
+        d inum = Some file ->
+        file.(owner) = u ->
+        let new_file := Build_File file.(owner) (file.(blocks) ++ [v]) in
+        exec' [Cont] s (Extend inum v) (Finished (u, (upd d inum new_file)) (Some tt))
+
+  | ExecExtendFail :
+      forall s inum file v,
+        let u := fst s in
+        let d := snd s in
+        (inum >= disk_size \/
+         d inum = None \/
+         (d inum = Some file /\ file.(owner) <> u)) ->
+        exec' [Cont] s (Extend inum v) (Finished s None)
+              
+  | ExecExtendFailDiskFull :
+      forall s inum file v,
+        let u := fst s in
+        let d := snd s in
+        inum < disk_size ->
+        d inum = Some file ->
+        file.(owner) = u ->
+        exec' [DiskFull] s (Extend inum v) (Finished s None)
+
+  | ExecSetOwnerSuccess :
+      forall s inum file o,
+        let u := fst s in
+        let d := snd s in
+        inum < disk_size ->
+        d inum = Some file ->
+        file.(owner) = u ->
+        let new_file := Build_File o file.(blocks) in
+        exec' [Cont] s (SetOwner inum o) (Finished (u, (upd d inum new_file)) (Some tt))
+
+  | ExecSetOwnerFail :
+      forall s inum file o,
+        let u := fst s in
+        let d := snd s in
+        (inum >= disk_size \/
+         d inum = None \/
+         (d inum = Some file /\ file.(owner) <> u)) ->
+        exec' [Cont] s (SetOwner inum o) (Finished s None)
+
+  | ExecCreateSuccess :
+      forall s inum owner,
+        let u := fst s in
+        let d := snd s in
+        inum < disk_size ->
+        d inum = None ->
+        let new_file := Build_File owner [] in
+        exec' [NewInum inum] s (Create owner) (Finished (u, (upd d inum new_file)) (Some inum))
+
+  | ExecCreateFail :
+      forall s owner,
+        let u := fst s in
+        let d := snd s in
+        (forall inum, inum < disk_size -> d inum <> None) ->
+        exec' [InodesFull] s (Create owner) (Finished s None)
+              
+  | ExecDeleteSuccess :
+      forall s inum file,
+        let u := fst s in
+        let d := snd s in
+        inum < disk_size ->
+        d inum = Some file ->
+        file.(owner) = u ->
+        exec' [Cont] s (Delete inum) (Finished (u, (Mem.delete d inum)) (Some tt))
+
+  | ExecDeleteFail :
+      forall s file inum,
+        let u := fst s in
+        let d := snd s in
+        (inum >= disk_size \/
+         d inum = None \/
+         (d inum = Some file /\ file.(owner) <> u)) ->
+        exec' [Cont] s (Delete inum) (Finished s None)
+
+  | ExecCrashBefore :
+      forall d T (p: file_disk_prog T),
+        exec' [CrashBefore] d p (Crashed d)
+
+  | ExecCrashAfter :
+      forall d T (p: file_disk_prog T) d' r o,
+        o = [Cont] \/ o = [InodesFull] ->
+        exec' o d p (Finished d' r) ->
+        exec' [CrashAfter] d p (Crashed d')
+
+  | ExecCreateCrashAfter :
+      forall s inum owner,
+        let u := fst s in
+        let d := snd s in
+        inum < disk_size ->
+        d inum = None ->
+        let new_file := Build_File owner [] in
+        exec' [CrashAfterCreate inum] s (Create owner) (Crashed (u, (upd d inum new_file))).
+
+  Hint Constructors exec' : core.
+
+  Definition weakest_precondition' T (p: file_disk_prog T) :=
+    match p in file_disk_prog T' return (T' -> state' -> Prop) -> oracle' -> state' -> Prop with
+    | Read inum a =>
+      fun Q o s =>
+        let u := fst s in
+        let d := snd s in
+        (
+          o = [Cont] /\
+          inum < disk_size /\
+          exists file v,
+            d inum = Some file /\
+            nth_error file.(blocks) a = Some v /\
+            file.(owner) = u /\
+            Q (Some v) s
+        ) \/
+        (
+          o = [Cont] /\
+          (inum >= disk_size \/
+           d inum = None \/
+           (exists file,
+              d inum = Some file /\
+              (
+                file.(owner) <> u \/
+                nth_error file.(blocks) a = None
+              )
+           )
+          ) /\
+          Q None s
+        )
+          
+    | Write inum a v =>
+      fun Q o s =>
+        let u := fst s in
+        let d := snd s in
+        (
+          o = [Cont] /\
+          inum < disk_size /\  
+          exists file,
+            d inum = Some file /\
+            file.(owner) = u /\
+            a < length (file.(blocks)) /\
+            let new_file :=
+                Build_File file.(owner)
+                                  (firstn a file.(blocks) ++ v :: skipn (S a) file.(blocks)) in
+            Q (Some tt) (u, upd d inum new_file)
+        ) \/
+        (
+          o = [Cont] /\
+          (inum >= disk_size \/
+           d inum = None \/
+           (exists file,
+              d inum = Some file /\
+              (
+                file.(owner) <> u \/
+                a >= length (file.(blocks))
+              )
+           )
+          ) /\
+          Q None s
+        )
+          
+    | SetOwner inum u' =>
+      fun Q o s =>
+        let u := fst s in
+        let d := snd s in
+        (
+          o = [Cont] /\
+          inum < disk_size /\
+          exists file,
+            let new_file := Build_File u' file.(blocks) in
+            d inum = Some file /\
+            file.(owner) = u /\
+            Q (Some tt) (u, upd d inum new_file)
+        ) \/
+        (
+          o = [Cont] /\
+          (inum >= disk_size \/ d inum = None \/
+           exists file,
+             d inum = Some file /\
+             file.(owner) <> u) /\
+          Q None s
+        )
+          
+    | Create u' =>
+      fun Q o s =>
+        let u := fst s in
+        let d := snd s in
+        (
+          o = [InodesFull] /\
+          (forall inum, inum < disk_size -> d inum <> None) /\
+          Q None s
+        ) \/
+
+        (exists inum,
+           o = [NewInum inum] /\
+           inum < disk_size /\ 
+           d inum = None /\
+           let new_file := Build_File u' [] in
+           Q (Some inum) (u, upd d inum new_file)
+        )
+          
+    | Delete inum =>
+      fun Q o s =>
+        let u := fst s in
+        let d := snd s in
+        (
+          o = [Cont] /\
+          inum < disk_size /\
+          (exists file,
+             d inum = Some file /\ 
+             file.(owner) = u) /\
+          Q (Some tt) (u, Mem.delete d inum)
+        ) \/
+        (
+          o = [Cont] /\
+          (inum >= disk_size \/
+           d inum = None \/
+           exists file,
+             d inum = Some file /\
+             file.(owner) <> u) /\
+          Q None s
+        )
+    | Extend inum v =>
+      fun Q o s =>
+        let u := fst s in
+        let d := snd s in
+        (
+          o = [DiskFull] /\
+          inum < disk_size /\
+          (exists file,
+             d inum = Some file /\ 
+             file.(owner) = u) /\
+          Q None s
+        ) \/
+        (
+          o = [Cont] /\
+          inum < disk_size /\
+          exists file,
+            d inum = Some file /\
+            file.(owner) = u /\
+            let new_file := Build_File file.(owner) (file.(blocks) ++ [v]) in
+            Q (Some tt) (u, upd d inum new_file)
+        ) \/
+        (
+          o = [Cont] /\
+          (inum >= disk_size \/ d inum = None \/
+           exists file,
+             d inum = Some file /\
+             file.(owner) <> u) /\
+          Q None s
+        )
+    end.
+
+  
+  Definition weakest_crash_precondition' T (p: file_disk_prog T) :=
+    match p in file_disk_prog T' return (state' -> Prop) -> oracle' -> state' -> Prop with
+    | Read inum a =>
+      fun Q o s =>
+        let u := fst s in
+        let d := snd s in
+        (
+          o = [CrashBefore] /\
+          Q s
+        ) \/
+        (
+          o = [CrashAfter] /\
+          inum < disk_size /\
+          exists file v,
+            d inum = Some file /\
+            file.(owner) = u /\
+            nth_error file.(blocks) a = Some v /\
+            Q s
+        ) \/
+        (
+          o = [CrashAfter] /\
+          (inum >= disk_size \/
+           d inum = None \/
+           (exists file,
+              d inum = Some file /\
+              (
+                file.(owner) <> u \/
+                nth_error file.(blocks) a = None
+              )
+           )
+          ) /\
+          Q s
+        )
+          
+    | Write inum a v =>
+      fun Q o s =>
+        let u := fst s in
+        let d := snd s in
+        (
+          o = [CrashBefore] /\
+          Q s
+        ) \/
+        (
+          o = [CrashAfter] /\
+          inum < disk_size /\  
+          exists file,
+            d inum = Some file /\
+            file.(owner) = u /\
+            a < length (file.(blocks)) /\
+            let new_file :=
+                Build_File file.(owner)
+                                  (firstn a file.(blocks) ++ v :: skipn (S a) file.(blocks)) in
+            Q (u, upd d inum new_file)
+        ) \/
+        (
+          o = [CrashAfter] /\
+          (inum >= disk_size \/
+           d inum = None \/
+           (exists file,
+              d inum = Some file /\
+              (
+                file.(owner) <> u \/
+                a >= length (file.(blocks))
+              )
+           )
+          ) /\
+          Q s
+        )
+          
+    | SetOwner inum u' =>
+      fun Q o s =>
+        let u := fst s in
+        let d := snd s in
+        (
+          o = [CrashBefore] /\
+          Q s
+        ) \/
+        (
+          o = [CrashAfter] /\
+          inum < disk_size /\
+          exists file,
+            let new_file := Build_File u' file.(blocks) in
+            d inum = Some file /\
+            file.(owner) = u /\
+            Q (u, upd d inum new_file)
+        ) \/
+        (
+          o = [CrashAfter] /\
+          (inum >= disk_size \/
+           d inum = None \/
+           exists file,
+             d inum = Some file /\
+             file.(owner) <> u) /\
+          Q s
+        )
+          
+    | Create u' =>
+      fun Q o s =>
+        let u := fst s in
+        let d := snd s in
+        (
+          o = [CrashBefore] /\
+          Q s
+        ) \/
+        (
+          o = [CrashAfter] /\
+          (forall inum, inum < disk_size -> d inum <> None) /\
+          Q s
+        ) \/
+
+        (exists inum,
+           o = [CrashAfterCreate inum] /\
+           inum < disk_size /\ 
+           d inum = None /\
+           let new_file := Build_File u' [] in
+           Q (u, upd d inum new_file)
+        )
+          
+    | Delete inum =>
+      fun Q o s =>
+        let u := fst s in
+        let d := snd s in
+        (
+          o = [CrashBefore] /\
+          Q s
+        ) \/
+        (
+          o = [CrashAfter] /\
+          inum < disk_size /\
+          (exists file,
+             d inum = Some file /\
+             file.(owner) = u) /\
+          Q (u, Mem.delete d inum)
+        ) \/
+        (
+          o = [CrashAfter] /\
+          (inum >= disk_size \/
+           d inum = None \/
+           exists file,
+             d inum = Some file /\
+             file.(owner) <> u) /\
+          Q s
+        )
+    | Extend inum v =>
+      fun Q o s =>
+        let u := fst s in
+        let d := snd s in
+        (
+          o = [CrashBefore] /\
+          Q s
+        ) \/
+        (
+          o = [CrashAfter] /\
+          inum < disk_size /\
+          exists file,
+            d inum = Some file /\
+            file.(owner) = u /\
+            let new_file := Build_File file.(owner) (file.(blocks) ++ [v]) in
+            Q (u, upd d inum new_file)
+        ) \/
+        (
+          o = [CrashAfter] /\
+          (inum >= disk_size \/
+           d inum = None \/
+           exists file,
+             d inum = Some file /\
+             file.(owner) <> u) /\
+          Q s
+        )
+    end.
+
+  Definition strongest_postcondition' T (p: file_disk_prog T) :=
+    match p in file_disk_prog T' return (oracle' -> state' -> Prop) -> T' -> state' -> Prop with
+    | Read inum a =>
+      fun P t s' =>
+        (
+          exists s,
+            let u := fst s in
+            let d := snd s in
+            P [Cont] s /\
+            inum < disk_size /\
+            exists file v,
+              d inum = Some file /\
+              file.(owner) = u /\
+              nth_error file.(blocks) a = Some v /\
+              t = Some v /\
+              s' = s
+        ) \/
+        (
+          exists s,
+            let u := fst s in
+            let d := snd s in
+            P [Cont] s /\
+            (inum >= disk_size \/
+             d inum = None \/
+             (exists file,
+                d inum = Some file /\
+                (
+                  file.(owner) <> u \/
+                  nth_error file.(blocks) a = None
+                )
+             )
+            ) /\
+            t = None /\
+            s' = s
+        )
+          
+    | Write inum a v =>
+      fun P t s' =>
+        (
+          exists s,
+            let u := fst s in
+            let d := snd s in
+            P [Cont] s /\
+            inum < disk_size /\  
+            exists file,
+              d inum = Some file /\
+              file.(owner) = u /\
+              a < length (file.(blocks)) /\
+              let new_file :=
+                  Build_File file.(owner)
+                                    (firstn a file.(blocks) ++ v :: skipn (S a) file.(blocks)) in
+              t = (Some tt) /\
+              s' = (u, upd d inum new_file)
+        ) \/
+        (
+          exists s,
+            let u := fst s in
+            let d := snd s in
+            P [Cont] s /\
+            (inum >= disk_size \/
+             d inum = None \/
+             (exists file,
+                d inum = Some file /\
+                (
+                  file.(owner) <> u \/
+                  a >= length (file.(blocks))
+                )
+             )
+            ) /\
+            t = None /\
+            s' = s
+        )
+          
+    | SetOwner inum u' =>
+      fun P t s' =>
+        (exists s,
+           let u := fst s in
+           let d := snd s in
+           P [Cont] s /\
+           inum < disk_size /\
+           exists file,
+             let new_file := Build_File u' file.(blocks) in
+             d inum = Some file /\
+             file.(owner) = u /\
+             t = (Some tt) /\
+             s' = (u, upd d inum new_file)
+        ) \/
+        (exists s,
+           let u := fst s in
+           let d := snd s in
+           P [Cont] s /\
+           (inum >= disk_size \/
+            d inum = None \/
+            exists file,
+              d inum = Some file /\
+              file.(owner) <> u) /\
+           t = None /\
+           s' = s
+        )
+          
+    | Create u' =>
+      fun P t s' =>
+        (exists s,
+           let u := fst s in
+           let d := snd s in
+           P [InodesFull] s /\
+           (forall inum, inum < disk_size -> d inum <> None) /\
+           t = None /\
+           s' = s
+        ) \/
+        (exists s inum,
+           let u := fst s in
+           let d := snd s in
+           P [NewInum inum] s /\
+           inum < disk_size /\ 
+           d inum = None /\
+           let new_file := Build_File u' [] in
+           t = (Some inum) /\
+           s' = (u, upd d inum new_file)
+        )
+          
+    | Delete inum =>
+      fun P t s' =>
+        (
+          exists s,
+            let u := fst s in
+            let d := snd s in
+            P [Cont] s /\
+            inum < disk_size /\
+            (exists file,
+               d inum = Some file /\
+               file.(owner) = u
+            ) /\
+            t = (Some tt) /\
+            s' = (u, Mem.delete d inum)
+        ) \/
+        (exists s,
+           let u := fst s in
+           let d := snd s in
+           P [Cont] s /\
+           (inum >= disk_size \/
+            d inum = None \/
+            exists file,
+              d inum = Some file /\
+              file.(owner) <> u) /\
+           t = None /\
+           s' = s
+        )
+          
+    | Extend inum v =>
+      fun P t s' =>
+        (exists s,
+           let u := fst s in
+           let d := snd s in
+           P [DiskFull] s /\
+           inum < disk_size /\
+           (exists file,
+              d inum = Some file /\
+              file.(owner) = u) /\
+           t = None /\
+           s' = s
+        ) \/
+        (exists s,
+           let u := fst s in
+           let d := snd s in
+           P [Cont] s /\
+           inum < disk_size /\
+           exists file,
+             d inum = Some file /\
+             file.(owner) = u /\
+             let new_file := Build_File file.(owner) (file.(blocks) ++ [v]) in
+             t = (Some tt) /\
+             s' = (u, upd d inum new_file)
+        ) \/
+        (exists s,
+           let u := fst s in
+           let d := snd s in
+           P [Cont] s /\
+           (inum >= disk_size \/
+            d inum = None \/
+            exists file,
+              d inum = Some file /\
+              file.(owner) <> u) /\
+           t = None /\
+           s' = s
+        )
+    end.
+  
+  Definition strongest_crash_postcondition' T (p: file_disk_prog T) :=
+    match p in file_disk_prog T' return (oracle' -> state' -> Prop) -> state' -> Prop with
+    | Read inum a =>
+      fun P s' =>
+        (exists s,
+           P [CrashBefore] s /\
+           s' = s
+        ) \/
+        (exists s,
+           let u := fst s in
+           let d := snd s in
+           P [CrashAfter] s /\
+           inum < disk_size /\
+           exists file v,
+             d inum = Some file /\
+             file.(owner) = u /\
+             nth_error file.(blocks) a = Some v /\
+             s' = s
+        ) \/
+        (exists s,
+           let u := fst s in
+           let d := snd s in
+           P [CrashAfter] s /\
+           (inum >= disk_size \/
+            d inum = None \/
+            (exists file,
+               d inum = Some file /\
+               (
+                 file.(owner) <> u \/
+                 nth_error file.(blocks) a = None
+               )
+            )
+           ) /\
+           s' = s
+        )
+          
+    | Write inum a v =>
+      fun P s' =>
+        (exists s,
+           P [CrashBefore] s /\
+           s' = s
+        ) \/
+        (exists s,
+           let u := fst s in
+           let d := snd s in
+           P [CrashAfter] s /\
+           inum < disk_size /\  
+           exists file,
+             d inum = Some file /\
+             file.(owner) = u /\
+             a < length (file.(blocks)) /\
+             let new_file :=
+                 Build_File file.(owner)
+                                   (firstn a file.(blocks) ++ v :: skipn (S a) file.(blocks)) in
+             s' = (u, upd d inum new_file)
+        ) \/
+        (exists s,
+           let u := fst s in
+           let d := snd s in
+           P [CrashAfter] s /\
+           (inum >= disk_size \/
+            d inum = None \/
+            (exists file,
+               d inum = Some file /\
+               (
+                 file.(owner) <> u \/
+                 a >= length (file.(blocks))
+               )
+            )
+           ) /\
+           s' = s
+        )
+          
+    | SetOwner inum u' =>
+      fun P s' =>
+        (exists s,
+           P [CrashBefore] s /\
+           s' = s
+        ) \/
+        (exists s,
+           let u := fst s in
+           let d := snd s in
+           P [CrashAfter] s /\
+           inum < disk_size /\
+           exists file,
+             let new_file := Build_File u' file.(blocks) in
+             d inum = Some file /\
+             file.(owner) = u /\
+             s' = (u, upd d inum new_file)
+        ) \/
+        (exists s,
+           let u := fst s in
+           let d := snd s in
+           P [CrashAfter] s /\
+           (inum >= disk_size \/ d inum = None \/
+            exists file,
+              d inum = Some file /\
+              file.(owner) <> u) /\
+           s' = s
+        )
+          
+    | Create u' =>
+      fun P s' =>
+        (exists s,
+           P [CrashBefore] s /\
+           s' = s
+        ) \/
+        (exists s,
+           let u := fst s in
+           let d := snd s in
+           P [CrashAfter] s /\
+           (forall inum, inum < disk_size -> d inum <> None) /\
+           s' = s
+        ) \/
+
+        (exists s inum,
+           let u := fst s in
+           let d := snd s in
+           P [CrashAfterCreate inum] s /\
+           inum < disk_size /\ 
+           d inum = None /\
+           let new_file := Build_File u' [] in
+           s' = (u, upd d inum new_file)
+        )
+          
+    | Delete inum =>
+      fun P s' =>
+        (exists s,
+           P [CrashBefore] s /\
+           s' = s
+        ) \/
+        (exists s,
+           let u := fst s in
+           let d := snd s in
+           P [CrashAfter] s /\
+           inum < disk_size /\
+           (exists file,
+              d inum = Some file /\
+             file.(owner) = u) /\
+           s' = (u, Mem.delete d inum)
+        ) \/
+        (exists s,
+           let u := fst s in
+           let d := snd s in
+           P [CrashAfter] s /\
+           (inum >= disk_size \/ d inum = None \/
+            exists file,
+              d inum = Some file /\
+              file.(owner) <> u) /\
+           s' = s
+        )
+    | Extend inum v =>
+      fun P s' =>
+        (exists s,
+           P [CrashBefore] s /\
+           s' = s
+        ) \/
+        (exists s,
+           let u := fst s in
+           let d := snd s in
+           P [CrashAfter] s /\
+           inum < disk_size /\
+           exists file,
+             d inum = Some file /\
+             file.(owner) = u /\
+             let new_file := Build_File file.(owner) (file.(blocks) ++ [v]) in
+             s' = (u, upd d inum new_file)
+        ) \/
+        (exists s,
+           let u := fst s in
+           let d := snd s in
+           P [CrashAfter] s /\
+           (inum >= disk_size \/ d inum = None \/
+            exists file,
+              d inum = Some file /\
+              file.(owner) <> u) /\
+           s' = s
+        )
+    end.
+
+  Arguments skipn : simpl never.
+  Theorem sp_complete':
+    forall T (p: file_disk_prog T) P (Q: _ -> _ -> Prop),
+      (forall t s', strongest_postcondition' p P t s' -> Q t s') <->
+      (forall o s s' t, P o s -> exec' o s p (Finished s' t) -> Q t s').
+  Proof.
+    intros; destruct p; simpl; eauto;
+    split; intros;
+    repeat (split_ors; cleanup; eauto);
+    eapply H; eauto;
+    try match goal with
+        | [H: exec' _ _ _ _ |- _] =>
+          inversion H; clear H; cleanup
+        end;
+    try solve [left; eexists; intuition eauto;               
+               repeat eexists; intuition eauto; cleanup; simpl; eauto ];
+    try solve [right; repeat eexists; intuition eauto ];
+    try solve [intuition eauto;
+               repeat eexists; intuition eauto;
+               try solve [ econstructor; eauto ];
+               simpl; cleanup; eauto ];
+    rewrite <- H3 at 2; eauto.
+    
+    Unshelve.
+    all: repeat econstructor; eauto.
+    all: exact user0.
+  Qed.
+
+  Theorem scp_complete':
+    forall T (p: file_disk_prog T) P (Q:  _ -> Prop),
+      (forall s', strongest_crash_postcondition' p P s' -> Q s') <->
+      (forall o s s', P o s -> exec' o s p (Crashed s') -> Q s').
+  Proof.
+    intros; destruct p; simpl; eauto;
+    split; intros;
+    repeat (split_ors; cleanup);
+    eapply H; eauto;
+    repeat
+      match goal with
+      | [H: exec' _ _ _ _ |- _] =>
+        inversion H; clear H; cleanup
+      end;
+    try solve [left; eexists; intuition eauto;               
+               repeat eexists; intuition eauto; cleanup; simpl; eauto ];
+    try solve [right; repeat eexists; intuition eauto ];
+    try solve [intuition eauto;
+               repeat eexists; intuition eauto;
+               try solve [
+                     econstructor;
+                     [| try solve [
+                              try rewrite <- H3 at 2;
+                              econstructor;  eauto
+                            ]
+                     ]; eauto
+                   ];
+               simpl; cleanup; eauto
+              ].
+    
+    Unshelve.
+    all: repeat econstructor; eauto.
+    all: exact user0.
+  Qed.
+  
+    Theorem wp_complete':
+    forall T (p: file_disk_prog T) H Q,
+      (forall o s, H o s -> weakest_precondition' p Q o s) <->
+      (forall o s, H o s -> (exists s' v, exec' o s p (Finished s' v) /\ Q v s')).
+  Proof.
+    intros; destruct p; simpl; eauto;
+    split; intros;
+    specialize H0 with (1:= X);
+    cleanup; eauto;
+    try match goal with
+        | [H: exec' _ _ _ _ |- _] =>
+          inversion H; clear H; cleanup
+        end;
+    try solve [
+          repeat (split_ors; cleanup; eauto);
+          do 2 eexists; intuition eauto;
+          try solve [ econstructor; eauto ];
+          simpl; cleanup; eauto ];
+    try solve [
+          left; intuition eauto;
+          do 2 eexists; intuition eauto;
+          try solve [ econstructor; eauto ];
+          simpl; cleanup; eauto ];
+    try solve [
+          right;intuition eauto;
+          do 2 eexists; intuition eauto;
+          try solve [ econstructor; eauto ];
+          simpl; cleanup; eauto ].
+    
+    Unshelve.
+    all: repeat econstructor; eauto.
+    all: exact user0.
+  Qed.
+  
+  Theorem wcp_complete':
+    forall T (p: file_disk_prog T) H C,
+      (forall o s, H o s -> weakest_crash_precondition' p C o s) <->
+      (forall o s, H o s -> (exists s', exec' o s p (Crashed s') /\ C s')).
+  Proof.
+    unfold weakest_crash_precondition';
+    intros; destruct p; simpl; eauto;
+    split; intros;
+    specialize H0 with (1:= X);
+    cleanup; eauto;
+    try repeat
+        match goal with
+        | [H: exec' _ _ _ _ |- _] =>
+          inversion H; clear H; cleanup
+        end;
+
+    try solve [
+          repeat (split_ors; cleanup; eauto);
+          repeat eexists; intuition eauto;
+          try solve [ repeat econstructor; eauto; congruence ];
+          try congruence; simpl; cleanup; eauto ];
+    try solve [
+          left; intuition eauto;
+          repeat eexists; intuition eauto;
+          try solve [ econstructor; eauto ];
+          simpl; cleanup; eauto ];
+    try solve [
+          right;intuition eauto;
+          repeat eexists; intuition eauto;
+          try solve [ econstructor; eauto ];
+          simpl; cleanup; eauto ].
+    
+    Unshelve.
+    all: repeat econstructor; eauto.
+    all: exact user0.
+  Qed.
+
+  Theorem exec_deterministic_wrt_oracle' :
+    forall o s T (p: file_disk_prog T) ret1 ret2,
+      exec' o s p ret1 ->
+      exec' o s p ret2 ->
+      ret1 = ret2.
+  Proof.
+    intros; destruct p; simpl in *; cleanup;
+    repeat
+      match goal with
+      | [H: exec' _ _ _ _ |- _] =>
+        inversion H; clear H; try split_ors; cleanup
+      end;
+    try solve [ repeat (cleanup; intuition eauto; try congruence; try omega) ].
+  Qed.
+  
+  Definition FileDiskOperation :=
+    Build_Operation
+      (list_eq_dec token_dec')
+      file_disk_prog
+      exec'
+      weakest_precondition'
+      weakest_crash_precondition'
+      strongest_postcondition'
+      strongest_crash_postcondition'
+      wp_complete'
+      wcp_complete'
+      sp_complete'
+      scp_complete'
+      exec_deterministic_wrt_oracle'.
+
+  Definition FileDiskLang := Build_Language FileDiskOperation.
+  Definition FileDiskHL := Build_HoareLogic FileDiskLang.
+
+End FileDisk.
+
+Notation "| p |" := (Op (FileDiskOperation _) p)(at level 60).
+Notation "x <-| p1 ; p2" := (Bind (Op (FileDiskOperation _) p1) (fun x => p2))(right associativity, at level 60). 
+Notation "p >> s" := (p s) (right associativity, at level 60, only parsing).
