src/Layers/AbstractLayers/TransactionalDisk/TransactionalDiskLayer.v
@@ -1,0 +1,463 @@
+Require Import Omega Framework.
+Import ListNotations.
+
+Set Implicit Arguments.
+
+Section TransactionalDisk.
+
+  Variable disk_size: nat.
+
+  Inductive token' :=
+  | CrashBefore : token'
+  | CrashAfter : token'
+  | Cont : token'
+  | TxnFull : token'.
+
+  Definition token_dec' : forall (t t': token'), {t=t'}+{t<>t'}.
+    decide equality.
+  Defined.
+
+  Definition oracle' := list token'.  
+
+  Definition state' := ((disk value) * (disk (set value)))%type.
+  
+  Inductive transactional_disk_prog : Type -> Type :=
+  | Start : transactional_disk_prog unit
+  | Read : addr -> transactional_disk_prog value
+  | Write : addr -> value -> transactional_disk_prog unit
+  | Commit : transactional_disk_prog unit
+  | Abort : transactional_disk_prog unit.
+   
+  Inductive exec' :
+    forall T, oracle' ->  state' -> transactional_disk_prog T -> @Result state' T -> Prop :=
+  | ExecStart : 
+      forall s,
+        let c := fst s in
+        let d := snd s in
+        exec' [Cont] s Start (Finished (empty_mem, d) tt)
+              
+  | ExecReadInbound : 
+      forall s a v,
+        let c := fst s in
+        let d := snd s in
+        a < disk_size ->
+        (c a = Some v \/
+        (c a = None /\ read d a = Some v)) ->
+        exec' [Cont] s (Read a) (Finished s v)
+
+  | ExecReadOutbound : 
+      forall s a,
+        a >= disk_size ->
+        exec' [Cont] s (Read a) (Finished s value0)
+             
+  | ExecWriteInbound :
+      forall s a v,
+        let c := fst s in
+        let d := snd s in
+        a < disk_size ->
+        exec' [Cont] s (Write a v) (Finished ((upd c a v), d) tt)
+
+  | ExecWriteInboundFull :
+      forall s a v,
+        a < disk_size ->
+        exec' [TxnFull] s (Write a v) (Finished s tt)
+              
+  | ExecWriteOutbound :
+      forall s a v,
+        a >= disk_size ->
+        exec' [Cont] s (Write a v) (Finished s tt)
+
+  | ExecCommit : 
+      forall s,
+        let c := fst s in
+        let d := snd s in
+        exec' [Cont] s Commit (Finished (empty_mem, merge c d) tt)
+
+  | ExecAbort : 
+      forall s,
+        let c := fst s in
+        let d := snd s in
+        exec' [Cont] s Abort (Finished (empty_mem, d) tt)
+
+  | ExecCrashBefore :
+      forall d T (p: transactional_disk_prog T),
+        exec' [CrashBefore] d p (Crashed d)
+
+  | ExecCrashAfter :
+      forall s s' T (p: transactional_disk_prog T),
+        (exists v, exec' [Cont] s p (Finished s' v)) ->
+        exec' [CrashAfter] s p (Crashed s').
+
+  Hint Constructors exec' : core.
+
+   Definition weakest_precondition' T (p: transactional_disk_prog T) :=
+   match p in transactional_disk_prog T' return (T' -> state' -> Prop) -> oracle' -> state' -> Prop with
+   | Start =>
+     (fun Q o s =>
+       let c := fst s in
+       let d := snd s in
+       o = [Cont] /\
+       Q tt (empty_mem, d))
+   | Read a =>
+     (fun Q o s =>
+        let c := fst s in
+        let d := snd s in
+        (
+          o = [Cont] /\
+          a < disk_size /\ 
+          exists v,
+            (c a = Some v \/ (c a = None /\ read d a = Some v)) /\
+            Q v s
+        ) \/
+        (
+          o = [Cont] /\
+          a >= disk_size /\
+          Q value0 s
+        )
+     )
+   | Write a v =>
+     (fun Q o s =>
+       let c := fst s in
+       let d := snd s in
+       
+       (
+         o = [Cont] /\
+         a < disk_size /\
+         Q tt ((upd c a v), d)
+       ) \/
+       (
+         o = [TxnFull] /\
+         a < disk_size /\
+         Q tt s
+       ) \/
+       (
+         o = [Cont] /\
+         a >= disk_size /\
+         Q tt s
+       )
+     )
+   | Commit =>
+     (fun Q o s =>
+       let c := fst s in
+       let d := snd s in
+       o = [Cont] /\
+       Q tt (empty_mem, merge c d))
+   | Abort =>
+     (fun Q o s =>
+       let c := fst s in
+       let d := snd s in
+       o = [Cont] /\
+       Q tt (empty_mem, d))
+   end.
+
+  Definition weakest_crash_precondition' T (p: transactional_disk_prog T) :=
+    match p in transactional_disk_prog T' return (state' -> Prop) -> oracle' -> state' -> Prop with
+    | Start =>
+      (fun Q o s =>
+         let c := fst s in
+         let d := snd s in
+         (o = [CrashBefore] /\
+          Q s) \/
+         (o = [CrashAfter] /\
+          Q (empty_mem, d)))
+   | Read a =>
+     (fun Q o s =>
+        let c := fst s in
+        let d := snd s in
+        (
+          o = [CrashBefore] /\
+          Q s
+        ) \/
+        (
+          o = [CrashAfter] /\
+          a < disk_size /\
+          Q s /\
+          exists v,
+            c a = Some v \/
+            (c a = None /\ read d a = Some v)
+        ) \/
+        (
+          o = [CrashAfter] /\
+          a >= disk_size /\
+          Q s
+        )
+     )
+   | Write a v =>
+     (fun Q o s =>
+        let c := fst s in
+        let d := snd s in
+        (
+          o = [CrashBefore] /\
+          Q s
+        ) \/
+        (
+          o = [CrashAfter] /\
+          a < disk_size /\
+          Q (upd c a v, d)
+        ) \/
+        (
+          o = [CrashAfter] /\
+          a >= disk_size /\
+          Q s
+        )
+     )
+   | Commit =>
+     (fun Q o s =>
+       let c := fst s in
+       let d := snd s in
+       (o = [CrashBefore] /\
+        Q s) \/
+       (o = [CrashAfter] /\
+        Q (empty_mem, merge c d)))
+   | Abort =>
+      (fun Q o s =>
+         let c := fst s in
+         let d := snd s in
+         (o = [CrashBefore] /\
+          Q s) \/
+         (o = [CrashAfter] /\
+          Q (empty_mem, d)))
+    end.
+
+  Definition strongest_postcondition' T (p: transactional_disk_prog T) :=
+    match p in transactional_disk_prog T' return (oracle' -> state' -> Prop) -> T' -> state' -> Prop with
+    | Start =>
+      fun P t s' =>
+        exists s,
+         let c := fst s in
+         let d := snd s in
+         P [Cont] s /\
+         t = tt /\
+         s' = (empty_mem, d)
+   | Read a =>
+     fun P t s' =>
+       exists s,
+         let c := fst s in
+         let d := snd s in
+         (
+           P [Cont] s /\
+           a < disk_size /\
+           s' = s /\
+           exists v,
+             ( c a = Some v \/ (c a = None /\ read d a = Some v) ) /\
+             t = v 
+         ) \/
+         (
+           P [Cont] s /\
+           s' = s /\
+           a >= disk_size /\
+           t = value0
+         )
+   | Write a v =>
+     fun P t s' =>
+       exists s,
+       let c := fst s in
+       let d := snd s in
+       (
+         P [Cont] s /\
+         a < disk_size /\
+         t = tt /\
+         s' = ((upd c a v), d)
+       ) \/
+       (
+         P [TxnFull] s /\
+         a < disk_size /\
+         t = tt /\
+         s' = s
+       ) \/
+       (
+         P [Cont] s /\
+         a >= disk_size /\
+         t = tt /\
+         s' = s
+       )
+         
+   | Commit =>
+      fun P t s' =>
+        exists s,
+         let c := fst s in
+         let d := snd s in
+         P [Cont] s /\
+         t = tt /\
+         s' = (empty_mem, merge c d)
+   | Abort =>
+      fun P t s' =>
+        exists s,
+         let c := fst s in
+         let d := snd s in
+         P [Cont] s /\
+         t = tt /\
+         s' = (empty_mem, d)
+   end.
+
+  Definition strongest_crash_postcondition' T (p: transactional_disk_prog T) :=
+    match p in transactional_disk_prog T' return (oracle' -> state' -> Prop) -> state' -> Prop with
+    | Start =>
+      fun P s' =>
+        exists s,
+          let c := fst s in
+          let d := snd s in
+          (P [CrashBefore] s /\
+           s' = s) \/
+          (P [CrashAfter] s /\
+           s' = (empty_mem, d))
+    | Read a =>
+     fun P s' =>
+       exists s,
+         let c := fst s in
+         let d := snd s in
+         (
+           P [CrashBefore] s /\
+           s' = s
+         ) \/
+         (
+           P [CrashAfter] s /\
+           a < disk_size /\
+           s' = s /\
+           (exists v, c a = Some v \/ (c a = None /\ read d a = Some v))
+         ) \/
+         (
+           P [CrashAfter] s /\
+           a >= disk_size /\
+           s' = s
+         )
+           
+   | Write a v =>
+     fun P s' =>
+       exists s,
+         let c := fst s in
+         let d := snd s in
+         (
+           P [CrashBefore] s /\
+           s' = s
+         ) \/
+         (
+           P [CrashAfter] s /\
+           a < disk_size /\
+           s' = (upd c a v, d)
+         ) \/
+         (
+           P [CrashAfter] s /\
+           a >= disk_size /\
+           s' = s
+         )
+           
+   | Commit =>
+      fun P s' =>
+       exists s,
+         let c := fst s in
+         let d := snd s in
+         (P [CrashBefore] s /\
+          s' = s) \/
+         (P [CrashAfter] s /\
+          s' = (empty_mem, merge c d))
+   | Abort =>
+      fun P s' =>
+        exists s,
+          let c := fst s in
+          let d := snd s in
+          (P [CrashBefore] s /\
+           s' = s) \/
+          (P [CrashAfter] s /\
+           s' = (empty_mem, d))
+    end.
+  
+  Theorem sp_complete':
+    forall T (p: transactional_disk_prog T) P (Q: _ -> _ -> Prop),
+      (forall t s', strongest_postcondition' p P t s' -> Q t s') <->
+      (forall o s s' t, P o s -> exec' o s p (Finished s' t) -> Q t s').
+  Proof.
+    intros; destruct p; simpl; eauto;
+    split; intros;
+    try match goal with
+        | [H: exec' _ _ _ _ |- _] =>
+          inversion H; clear H
+        end; cleanup;
+    try solve [ eapply H; eauto;
+    try solve [ repeat (eexists; intuition eauto) ];
+    try solve [ eexists; intuition eauto; eexists; intuition eauto ] ];
+    repeat split_ors; cleanup; eauto.
+  Qed.
+
+  Theorem scp_complete':
+    forall T (p: transactional_disk_prog T) P (Q:  _ -> Prop),
+      (forall s', strongest_crash_postcondition' p P s' -> Q s') <->
+      (forall o s s', P o s -> exec' o s p (Crashed s') -> Q s').
+  Proof.
+    intros; destruct p; simpl; eauto;
+    split; intros; cleanup;
+    repeat (try split_ors; try inversion H1; clear H1; cleanup; eauto);
+    try split_ors; cleanup;
+    try solve [ eapply H; eauto;
+    try solve [ eexists; right; intuition eauto];    
+    try solve [ split_ors; cleanup; econstructor; eauto ] ];
+    repeat split_ors; cleanup; eauto.
+  Qed.
+
+  Theorem wp_complete':
+    forall T (p: transactional_disk_prog T) H Q,
+      (forall o s, H o s -> weakest_precondition' p Q o s) <->
+      (forall o s, H o s -> (exists s' v, exec' o s p (Finished s' v) /\ Q v s')).
+  Proof.
+    intros; destruct p; simpl; eauto;
+    split; intros;
+    specialize H0 with (1:= X);
+    cleanup; eauto;
+    try inversion H0; cleanup; eauto.
+    intuition eauto.
+    repeat (split_ors; cleanup);
+    do 2 eexists; eauto.   
+  Qed.
+  
+  Theorem wcp_complete':
+    forall T (p: transactional_disk_prog T) H C,
+      (forall o s, H o s -> weakest_crash_precondition' p C o s) <->
+      (forall o s, H o s -> (exists s', exec' o s p (Crashed s') /\ C s')).
+  Proof.
+    unfold weakest_crash_precondition';
+    intros; destruct p; simpl; eauto;
+    split; intros; cleanup;
+    specialize H0 with (1:= X);
+    try split_ors; cleanup; repeat (try inversion H0; try clear H0; cleanup; eauto);
+    try solve [eexists; econstructor; eauto].
+    right; intuition eauto.
+  Qed.
+
+  Theorem exec_deterministic_wrt_oracle' :
+    forall o s T (p: transactional_disk_prog T) ret1 ret2,
+      exec' o s p ret1 ->
+      exec' o s p ret2 ->
+      ret1 = ret2.
+  Proof.
+    intros; destruct p; simpl in *; cleanup;
+    repeat
+      match goal with
+      | [H: exec' _ _ _ _ |- _] =>
+        inversion H; clear H; cleanup
+      end; eauto;
+    repeat split_ors; cleanup; eauto; omega.
+  Qed.
+  
+  Definition TransactionalDiskOperation :=
+    Build_Operation
+      (list_eq_dec token_dec')
+      transactional_disk_prog
+      exec'
+      weakest_precondition'
+      weakest_crash_precondition'
+      strongest_postcondition'
+      strongest_crash_postcondition'
+      wp_complete'
+      wcp_complete'
+      sp_complete'
+      scp_complete'
+      exec_deterministic_wrt_oracle'.
+
+  Definition TransactionalDiskLang := Build_Language TransactionalDiskOperation.
+  Definition TransactionalDiskHL := Build_HoareLogic TransactionalDiskLang.
+
+End TransactionalDisk.
+
+Notation "| p |" := (Op (TransactionalDiskOperation _) p)(at level 60).
+Notation "x <-| p1 ; p2" := (Bind (Op (TransactionalDiskOperation _) p1) (fun x => p2))(right associativity, at level 60). 
+Notation "p >> s" := (p s) (right associativity, at level 60, only parsing).
