src/Layers/ComposedLayers/AuthenticatedDisk/AuthenticatedDiskLayer.v
@@ -1,0 +1,14 @@
+Require Import FSParameters Framework.
+Require Export AuthenticationLayer TransactionalDiskLayer.
+Import ListNotations.
+
+Set Implicit Arguments.
+
+Definition AuthenticatedDiskOperation :=  HorizontalComposition AuthenticationOperation (TransactionalDiskOperation data_length).
+Definition AuthenticatedDiskLang := Build_Language AuthenticatedDiskOperation.
+Definition AuthenticatedDiskHL := Build_HoareLogic AuthenticatedDiskLang.
+
+Notation "'|ADAP|' p" := (@lift_L1 AuthenticationOperation (TransactionalDiskOperation data_length) AuthenticationLang _ p) (at level 59).
+Notation "'|ADDP|' p" := (@lift_L2 AuthenticationOperation (TransactionalDiskOperation data_length) (TransactionalDiskLang data_length) _ p) (at level 59).
+Notation "'|ADAO|' p" := (@lift_L1 AuthenticationOperation (TransactionalDiskOperation data_length) AuthenticationLang  _ (Op AuthenticationOperation p)) (at level 59).
+Notation "'|ADDO|' p" := (@lift_L2 AuthenticationOperation (TransactionalDiskOperation data_length) (TransactionalDiskLang data_length) _ (Op (TransactionalDiskOperation data_length) p)) (at level 59).
