src/Layers/LoggedDisk/LoggedDiskLayer.v
@@ -1,1 +1,0 @@
-Require Export Layers.LoggedDisk.Definitions.
