src/Layers/TransactionalDisk/TransactionalDiskLayer.v
@@ -1,1 +1,0 @@
-Require Export Layers.TransactionalDisk.Definitions.
