src/Noninterference/FileDiskNoninterference.v
@@ -1,0 +1,157 @@
+Require Import Framework File FileDiskLayer.
+
+Variable disk_size: nat.
+Notation "'FileDisk'" := (FileDiskLang disk_size) (at level 0).
+
+Definition same_for_user (s1 s2: FileDisk.(state)) :=
+  let u1 := fst s1 in
+  let u2 := fst s2 in
+  let d1 := snd s1 in
+  let d2 := snd s2 in
+  u1 = u2 /\
+  addrs_match d1 d2 /\
+  addrs_match d2 d1 /\
+  (forall inum file1 file2,
+     d1 inum = Some file1 ->
+     d2 inum = Some file2 ->
+     (file1.(owner) = u1 \/
+      file2.(owner) = u1) ->
+     file1 = file2) /\
+  (forall inum file1 file2,
+     d1 inum = Some file1 ->
+     d2 inum = Some file2 ->
+     file1.(owner) = file2.(owner) /\ 
+     length file1.(blocks) = length file2.(blocks)).
+
+Print SelfSimulation.
+
+(*
+
+Theorem self_simulation_from_wp :
+  forall O (L: Language O)
+    (valid_state: L.(state) -> Prop)
+    (valid_prog: forall T, L.(prog) T -> Prop)
+    (R: L.(state) -> L.(state) -> Prop), 
+
+    (forall T (p: L.(prog) T) (s1 s2: L.(state)) o s1' t1,
+       valid_state s1 ->
+       valid_state s2 ->
+       valid_prog T p ->
+       R s1 s2 ->
+       weakest_precondition L p (fun t' s' => R s1' s' /\ t' = t1) o s1 ->
+       exec L o s1 p (Finished s1' t1) ->
+       weakest_precondition L p (fun t' s' => R s1' s' /\ t' = t1) o s2) ->
+    SelfSimulation L valid_state valid_prog R.
+Proof.
+  intros.
+  constructor.
+  intros.
+  destruct s1'.
+  { (* Finished *)
+    eapply H in H3; eauto.
+    eapply wp_to_exec in H3; cleanup.
+    eexists; simpl; intuition eauto.
+    simpl.
+ *)
+
+Theorem Invariant_for_file_disk_read:
+  SelfSimulation FileDisk (fun _ => True) (fun T p => match p with
+                                             | Op _ o =>
+                                               match o with
+                                               | Read _ _ => True
+                                               |_ => False
+                                               end
+                                             | _ => False
+                                             end) same_for_user.
+Proof.
+  econstructor.
+  intros; destruct p; simpl in *; try tauto.  
+  destruct p; try tauto; cleanup.
+ 
+  invert_exec; cleanup.
+  { (* Read Worked *)
+    invert_exec; cleanup.
+    { (* Read successful *)
+      exists (Finished s2 (Some v)).
+      simpl; intuition eauto.
+      unfold same_for_user in *; cleanup.
+      specialize (H1 a).
+      destruct_fresh (snd s2 a); eauto; try congruence.
+      specialize (H3 a file f H9 D).
+      setoid_rewrite H0 in H10.        
+      rewrite H3 in *; eauto.
+      repeat (econstructor; eauto; simpl).
+      exfalso; apply H1; eauto; setoid_rewrite H9; congruence.
+    }          
+    { (* Read Failed *)
+      exists (Finished s2 None);        
+      simpl; split; [| intuition eauto].
+      econstructor; simpl.
+      repeat split_ors; cleanup;
+      try solve [eapply ExecReadFail; eauto].
+      
+      -
+        destruct_fresh (snd s2 a); eauto.
+        unfold same_for_user in *; cleanup.
+        specialize (H3 a).
+        exfalso; eapply H3; try congruence; eauto.
+        eapply ExecReadFail; eauto.
+      
+      - unfold same_for_user in *; cleanup.
+        specialize (H3 a).
+        destruct_fresh (snd s2 a); eauto; try congruence.
+        specialize (H5 a file f H0 D).
+        specialize (H6 a file f H0 D); cleanup.
+        eapply ExecReadFail; eauto.
+        right; right; intuition eauto.
+        left; intuition; cleanup; eauto.
+        right; apply nth_error_None.
+        rewrite <- H7; apply nth_error_None; eauto.
+        
+        exfalso; eapply H3; eauto;
+        setoid_rewrite H0; congruence.
+    }
+  }
+  { (* Read Crashed *)
+    exists (Crashed s2).
+    intuition eauto;
+    simpl; repeat invert_exec; cleanup; eauto.
+    { (* Crashed Before *)
+      repeat econstructor; eauto.
+    }
+    {
+      split_ors; cleanup;
+      inversion H8; cleanup.
+      -
+        repeat econstructor; eauto.
+        unfold same_for_user in *; cleanup.
+        specialize (H1 a).
+        destruct_fresh (snd s2 a); eauto; try congruence.
+        specialize (H3 a file f H6 D).
+        specialize (H4 a file f H6 D); cleanup.
+        rewrite H3 in *; eauto.        
+        exfalso; eapply H1; eauto;
+        setoid_rewrite H6; congruence.
+        
+        unfold same_for_user in *; cleanup; eauto.
+
+      - admit.
+    }
+    {
+      split_ors; cleanup;
+      inversion H8; cleanup; eauto.
+    }
+    Unshelve.
+    all: repeat constructor; eauto.
+    all: exact user0.
+Admitted.
+
+Axiom self_simulation_for_file_disk:
+  SelfSimulation FileDisk (fun _ => True) (fun _ _ => True) same_for_user.
+
+
+
+oracle_refines_to_same_from_related refinement same_for_user ->
+
+exec_compiled_preserves_validity refinement                           
+   (refines_to_valid refinement same_for_user).
