src/Refinements/FileToFileDisk/Refinement.v
@@ -1,0 +1,963 @@
+Require Import Framework FSParameters AuthenticatedDiskLayer FileDiskLayer.
+Require Import File FileToFileDisk.Definitions.
+Require Import ClassicalFacts FunctionalExtensionality Omega.
+
+Set Nested Proofs Allowed.
+
+Notation "'low'" := TransactionCacheLang.
+Notation "'high'" := (TransactionalDiskLang data_length).
+Notation "'refinement'" := TransactionalDiskRefinement.
+
+Section TransactionalDiskBisimulation.
+
+  Axiom exec_compiled_preserves_refinement:
+    exec_compiled_preserves_refinement refinement.
+
+  Axiom exec_preserves_refinement:
+    exec_preserves_refinement refinement.
+
+
+  Lemma merge_some_l:
+    forall AT AEQ V (m1: @mem AT AEQ V) m2 a v,
+      m1 a = Some v ->
+      m2 a <> None ->
+      exists vs, merge m1 m2 a = Some vs /\
+            fst vs = v.
+  Proof.
+    unfold merge; simpl; intros.
+    cleanup.
+    destruct (m2 a); try congruence; eauto.
+  Qed.
+  
+  Lemma merge_some_r:
+    forall AT AEQ V (m1: @mem AT AEQ V) m2 a,
+      m1 a = None ->
+      merge m1 m2 a = m2 a.
+  Proof.
+    unfold merge; simpl; intros.
+    cleanup; eauto.
+  Qed.
+
+  Lemma apply_list_app:
+    forall A AEQ V  l l' (m: @mem A AEQ V), 
+      apply_list m (l++l') =
+      apply_list (apply_list m l) l'.
+  Proof.
+    induction l; simpl; eauto.
+  Qed.
+  
+  Lemma apply_list_get_latest_eq :
+    forall l a,
+      get_latest l a = apply_list empty_mem (rev l) a.
+  Proof.
+    induction l; simpl; intros; eauto.
+    rewrite apply_list_app; simpl.
+    destruct (addr_eq_dec a0 (fst a)); subst.          
+    rewrite upd_eq; eauto.
+    rewrite upd_ne; eauto.
+  Qed.
+
+  Lemma empty_mem_some_false:
+    forall A AEQ V (m: @mem A AEQ V) a v,
+      m = empty_mem ->
+      m a <> Some v.
+  Proof.
+    intros.
+    rewrite H.
+    unfold empty_mem; simpl; congruence.
+  Qed.
+
+  
+  Lemma refines_to_upd:
+    forall s1 s2 a vl,
+      fst s1 <> None ->
+      refines_to s1 s2 ->
+      refines_to (option_map (fun l : list (addr * value) => (a, vl) :: l) (fst s1), snd s1)
+                 (upd (fst s2) a vl, snd s2).
+  Proof.
+    unfold refines_to; intros;
+    cleanup; simpl in *; intuition.
+    destruct (fst s1); simpl in *; try congruence.
+    rewrite apply_list_app; simpl. eauto.
+  Qed.
+   
+  Lemma wp_low_to_high_read :
+    forall a,
+    wp_low_to_high_prog' _ _ _ _ refinement _ (|Read a|).
+  Proof.
+    unfold wp_low_to_high_prog', compilation_of; simpl; intros; cleanup.
+    unfold  compilation_of in *; simpl; intros; cleanup.
+    split_ors; cleanup; eapply exec_deterministic_wrt_oracle in H0; eauto; cleanup.
+    eexists; intuition eauto.
+    eapply exec_to_sp with (P := fun o s => refines_to s s2 /\ s = s1) in H3; eauto.
+
+    cleanup; simpl in *; cleanup; eauto;
+    eexists; intuition eauto; unfold refines_to in *; cleanup;
+    try congruence.      
+    rewrite apply_list_get_latest_eq in D0; eauto.
+    right; intuition.        
+    rewrite <- apply_list_get_latest_eq; eauto.
+    }
+    cleanup; eauto.
+    cleanup; simpl in *; cleanup.
+  Qed.
+
+  Lemma wp_high_to_low_read :
+    forall a,
+    wp_high_to_low_prog' _ _ _ _ refinement _ (|Read a|).
+  Proof.
+    unfold wp_high_to_low_prog', compilation_of; simpl; intros; cleanup.
+    unfold compilation_of in *; simpl; intros.
+    simpl in *; subst.
+    destruct H2; try solve [cleanup; split_ors; cleanup ].
+    cleanup.
+    repeat invert_exec.
+    cleanup.
+    eapply exec_to_wp; eauto; simpl.
+    split; eauto.
+    eapply exec_to_sp with (P := fun o s => refines_to s s2') in H; eauto.
+    unfold read in *; simpl in *.
+    cleanup; simpl in *.        
+    rewrite apply_list_get_latest_eq in H; cleanup; simpl in *; cleanup;
+    unfold refines_to in H; simpl in *; cleanup;    
+    repeat split_ors; cleanup; eauto;
+    try setoid_rewrite H2 in D; cleanup; eauto.
+    try setoid_rewrite H3 in D; cleanup; eauto.
+  Qed.
+
+  Lemma wcp_low_to_high_read :
+    forall a,
+    wcp_low_to_high_prog' _ _ _ _ refinement _ (|Read a|).
+  Proof.
+    unfold wcp_low_to_high_prog'; simpl; intros; cleanup.
+    unfold compilation_of in *; simpl in *; subst.
+    split_ors; cleanup; eapply exec_deterministic_wrt_oracle in H0; eauto; cleanup.
+
+    split_ors; cleanup; eauto.
+    eexists; intuition eauto.
+    - right; intuition eauto.
+      unfold refines_to in *; cleanup;
+      setoid_rewrite H2 in D; cleanup.
+      rewrite <- apply_list_get_latest_eq; eauto.
+    - right; intuition eauto.
+      unfold refines_to in *; cleanup;
+      setoid_rewrite H2 in D; cleanup.
+      rewrite <- apply_list_get_latest_eq; eauto.
+  Qed.
+
+  Lemma wcp_high_to_low_read :
+    forall a,
+    wcp_high_to_low_prog' _ _ _ _ refinement _ (|Read a|).
+  Proof.
+    unfold wcp_high_to_low_prog', compilation_of; simpl; intros; cleanup.
+    unfold compilation_of in *; simpl; intros; cleanup.
+    repeat (split_ors; cleanup);
+    repeat invert_exec;
+    cleanup;
+    repeat match goal with
+    | [H: Operation.exec _ _ _ _ _ |- _ ] =>
+      inversion H; clear H; cleanup
+    | [H: exec' _ _ _ _ |- _ ] =>
+      inversion H; clear H; cleanup
+    end;
+    eapply exec_to_wcp; eauto.
+  Qed.
+
+  Lemma wp_low_to_high_write :
+    forall a vl,
+    wp_low_to_high_prog' _ _ _ _ refinement _ (|Write a vl|).
+  Proof.
+    unfold wp_low_to_high_prog', compilation_of; simpl; intros; cleanup.
+    unfold compilation_of in *; simpl; intros; cleanup.
+    split_ors; cleanup; eapply exec_deterministic_wrt_oracle in H0; eauto; cleanup.
+    eapply exec_to_sp with (P := fun o s => refines_to s s2) in H3; eauto.
+    unfold write in *.
+    simpl in *; cleanup.
+    simpl in *; cleanup.
+    eexists; intuition eauto.
+    clear H1 H17; unfold refines_to in *; simpl in *; cleanup.
+    rewrite apply_list_app; eauto.
+  Qed.
+
+  Lemma wp_high_to_low_write :
+    forall a vl,
+    wp_high_to_low_prog' _ _ _ _ refinement _ (|Write a vl|).
+  Proof.
+    unfold wp_high_to_low_prog', compilation_of; simpl; intros; cleanup.
+    unfold compilation_of in *; simpl; intros; cleanup.
+    repeat invert_exec; cleanup.
+    repeat (split_ors; cleanup).
+    eapply exec_to_wp; simpl; eauto.
+    eapply exec_to_sp with (P := fun o s => refines_to s s2) in H; eauto.
+    unfold write in *.
+    simpl in *; cleanup.
+    eexists; intuition eauto.
+    clear H1; unfold refines_to in *; simpl in *; cleanup.
+    rewrite apply_list_app; eauto.
+    rewrite <- H1 at 1; rewrite apply_list_app; simpl; eauto.
+  Qed.
+
+  
+  Lemma wcp_low_to_high_write :
+    forall a vl,
+    wcp_low_to_high_prog' _ _ _ _ refinement _ (|Write a vl|).
+  Proof.
+    unfold wcp_low_to_high_prog', compilation_of; simpl; intros; cleanup.
+    unfold compilation_of in *; simpl; intros; cleanup.
+    split_ors; cleanup; eapply exec_deterministic_wrt_oracle in H0; eauto; cleanup.
+    split_ors; cleanup;
+    eexists; intuition eauto.
+
+    right; intuition eauto.
+    apply refines_to_upd; eauto.
+  Qed.
+
+  Lemma wcp_high_to_low_write :
+    forall a vl,
+    wcp_high_to_low_prog' _ _ _ _ refinement _ (|Write a vl|).
+  Proof.
+    unfold wcp_high_to_low_prog', compilation_of; simpl; intros; cleanup.
+    unfold compilation_of in *; simpl; intros; cleanup.
+    repeat split_ors; cleanup; repeat invert_exec;
+    try inversion H8; try clear H8; cleanup;
+    try inversion H9; try clear H9; cleanup;
+    eapply exec_to_wcp; eauto.
+    - split_ors; cleanup; eauto.
+      
+    - split_ors; cleanup; eauto.
+      repeat invert_exec;
+      repeat match goal with
+             | [H: Operation.exec _ _ _ _ _ |- _ ] =>
+               inversion H; clear H; cleanup
+             | [H: exec' _ _ _ _ |- _ ] =>
+               inversion H; clear H; cleanup
+             end.
+      eapply refines_to_upd; eauto.
+  Qed.
+
+  Lemma wp_low_to_high_start :
+    wp_low_to_high_prog' _ _ _ _ refinement _ (|Start|).
+  Proof.
+    unfold wp_low_to_high_prog', compilation_of; simpl; intros; cleanup.
+    unfold compilation_of in *; simpl in *; intros; cleanup.
+    split_ors; cleanup; eapply exec_deterministic_wrt_oracle in H0; eauto; cleanup.
+    eapply exec_to_sp with (P := fun o s => refines_to s s2) in H3; eauto.
+    simpl in *; cleanup.
+    eexists; intuition eauto.
+    clear H0 H9.
+    unfold refines_to in *; cleanup; eauto.
+  Qed.
+
+  Lemma wp_high_to_low_start :
+    wp_high_to_low_prog' _ _ _ _ refinement _ (|Start|).
+  Proof.
+    unfold wp_high_to_low_prog', compilation_of; simpl; intros; cleanup.
+    unfold compilation_of in *; simpl; intros; cleanup.
+    repeat (split_ors; cleanup).
+
+    repeat invert_exec; cleanup.    
+    eapply exec_to_wp; eauto.
+    eapply exec_to_sp with (P := fun o s => refines_to s s2) in H; eauto.
+    simpl in *; cleanup.
+    eexists; intuition eauto.
+    clear H H5.
+    unfold refines_to in *; cleanup; eauto.
+  Qed.
+
+  Lemma wcp_low_to_high_start :
+    wcp_low_to_high_prog' _ _ _ _ refinement _ (|Start|).
+  Proof.
+    unfold wcp_low_to_high_prog', compilation_of; simpl; intros; cleanup.
+    unfold compilation_of in *; simpl in *; intros; cleanup.
+    split_ors; cleanup; eapply exec_deterministic_wrt_oracle in H0; eauto; cleanup.
+    split_ors; cleanup; eauto.
+    eexists; intuition eauto.
+    right; unfold refines_to in *; cleanup; eauto.
+  Qed.
+
+  Lemma wcp_high_to_low_start :
+    wcp_high_to_low_prog' _ _ _ _ refinement _ (|Start|).
+  Proof.
+    unfold wcp_high_to_low_prog', compilation_of; simpl; intros; cleanup.
+    unfold compilation_of in *; simpl in *; intros; cleanup.
+    split_ors; cleanup.
+    repeat invert_exec.
+    eapply exec_to_wcp; eauto.
+    split_ors; cleanup.
+    repeat invert_exec; eauto.
+    repeat invert_exec; eauto.
+    cleanup.
+    repeat
+      match goal with
+      | [H: Operation.exec _ _ _ _ _ |- _ ] =>
+        inversion H; clear H; cleanup
+      | [H: exec' _ _ _ _ |- _ ] =>
+        inversion H; clear H; cleanup
+      end.
+    unfold refines_to in *; cleanup; eauto.
+  Qed.
+
+  
+  Lemma wp_low_to_high_abort :
+    wp_low_to_high_prog' _ _ _ _ refinement _ (|Abort|).
+  Proof.
+    unfold wp_low_to_high_prog', compilation_of; simpl; intros; cleanup.
+    unfold compilation_of in *; simpl in *; intros; cleanup.
+    split_ors; cleanup; eapply exec_deterministic_wrt_oracle in H0; eauto; cleanup.
+    eapply exec_to_sp with (P := fun o s => refines_to s s2) in H3; eauto.
+    simpl in *; cleanup.
+    eexists; intuition eauto.
+    clear H1 H9.
+    unfold refines_to in *; simpl in *; cleanup; eauto.
+  Qed.
+
+  Lemma wp_high_to_low_abort :
+    wp_high_to_low_prog' _ _ _ _ refinement _ (|Abort|).
+  Proof.
+    unfold wp_high_to_low_prog', compilation_of; simpl; intros; cleanup.
+    unfold compilation_of in *; simpl; intros; cleanup.
+    repeat (split_ors; cleanup).
+
+    repeat invert_exec; cleanup.    
+    eapply exec_to_wp; eauto.
+    eapply exec_to_sp with (P := fun o s => refines_to s s2) in H; eauto.
+    simpl in *; cleanup.
+    eexists; intuition eauto.
+    clear H1 H5.
+    unfold refines_to in *; simpl; cleanup; eauto.
+  Qed.
+
+  Lemma wcp_low_to_high_abort :
+    wcp_low_to_high_prog' _ _ _ _ refinement _ (|Abort|).
+  Proof.
+    unfold wcp_low_to_high_prog', compilation_of; simpl; intros; cleanup.
+    unfold compilation_of in *; simpl in *; intros; cleanup.
+    split_ors; cleanup; eapply exec_deterministic_wrt_oracle in H0; eauto; cleanup.
+    split_ors; cleanup; eauto.
+    eexists; intuition eauto.
+    right; unfold refines_to in *; cleanup; eauto.
+  Qed.
+
+  Lemma wcp_high_to_low_abort :
+    wcp_high_to_low_prog' _ _ _ _ refinement _ (|Abort|).
+  Proof.
+    unfold wcp_high_to_low_prog', compilation_of; simpl; intros; cleanup.
+    unfold compilation_of in *; simpl in *; intros; cleanup.
+    split_ors; cleanup.
+    repeat invert_exec.
+    eapply exec_to_wcp; eauto.
+    split_ors; cleanup.
+    repeat invert_exec; eauto.
+    repeat invert_exec; eauto.
+    cleanup.
+    repeat
+      match goal with
+      | [H: Operation.exec _ _ _ _ _ |- _ ] =>
+        inversion H; clear H; cleanup
+      | [H: exec' _ _ _ _ |- _ ] =>
+        inversion H; clear H; cleanup
+      end.
+    unfold refines_to in *; cleanup; eauto.
+  Qed.
+
+  
+  Lemma wp_low_to_high_commit :
+    wp_low_to_high_prog' _ _ _ _ refinement _ (|Commit|).
+  Proof.
+    unfold wp_low_to_high_prog', compilation_of; simpl; intros; cleanup.
+    unfold compilation_of in *; simpl in *; intros; cleanup.
+    split_ors; cleanup; eapply exec_deterministic_wrt_oracle in H0; eauto; cleanup.
+    eapply exec_to_sp with (P := fun o s => refines_to s s2) in H3; eauto.
+    simpl in *; cleanup.
+    eexists; intuition eauto.    
+    unfold refines_to; simpl; cleanup; eauto.
+    intuition.
+    unfold refines_to in H1; cleanup; intuition;
+    setoid_rewrite H14 in D; cleanup.
+    rewrite <- H7; eauto.
+  Qed.
+
+  Lemma wp_high_to_low_commit :
+    wp_high_to_low_prog' _ _ _ _ refinement _ (|Commit|).
+  Proof.
+    unfold wp_high_to_low_prog', compilation_of; simpl; intros; cleanup.
+    unfold compilation_of in *; simpl; intros; cleanup.
+    repeat (split_ors; cleanup).
+
+    repeat invert_exec; cleanup.    
+    eapply exec_to_wp; eauto.
+    eapply exec_to_sp with (P := fun o s => refines_to s s2) in H; eauto.
+    simpl in *; cleanup.
+    eexists; intuition eauto.
+    unfold refines_to; simpl; cleanup; eauto.
+    intuition.
+    unfold refines_to in H1; cleanup; intuition;
+    setoid_rewrite H2 in D; cleanup.
+    rewrite <- H7; eauto.
+  Qed.
+
+  Lemma wcp_low_to_high_commit :
+    wcp_low_to_high_prog' _ _ _ _ refinement _ (|Commit|).
+  Proof.
+    unfold wcp_low_to_high_prog', compilation_of; simpl; intros; cleanup.
+    unfold compilation_of in *; simpl in *; intros; cleanup.
+    split_ors; cleanup; eapply exec_deterministic_wrt_oracle in H0; eauto; cleanup.
+    split_ors; cleanup; eauto.
+    eexists; intuition eauto.
+    right; intuition eauto.
+    unfold refines_to; simpl; cleanup; eauto.
+    intuition.
+    unfold refines_to in H1; cleanup; intuition;
+    setoid_rewrite H2 in D; cleanup; eauto.
+  Qed.
+
+  Lemma wcp_high_to_low_commit :
+    wcp_high_to_low_prog' _ _ _ _ refinement _ (|Commit|).
+  Proof.
+    unfold wcp_high_to_low_prog', compilation_of; simpl; intros; cleanup.
+    unfold compilation_of in *; simpl in *; intros; cleanup.
+    split_ors; cleanup.
+    repeat invert_exec.
+    eapply exec_to_wcp; eauto.
+    split_ors; cleanup.
+    repeat invert_exec; eauto.
+    repeat invert_exec; eauto.
+    cleanup.
+    repeat
+      match goal with
+      | [H: Operation.exec _ _ _ _ _ |- _ ] =>
+        inversion H; clear H; cleanup
+      | [H: exec' _ _ _ _ |- _ ] =>
+        inversion H; clear H; cleanup
+      end.
+    unfold refines_to; simpl; cleanup; eauto.
+    clear H4; intuition.
+    unfold refines_to in H1; cleanup; intuition;
+    setoid_rewrite H2 in D; cleanup; eauto.
+  Qed.
+  
+
+  Lemma wp_low_to_high_ret :
+    forall T (v: T),
+    wp_low_to_high_prog' _ _ _ _ refinement _ (Ret v).
+  Proof.
+    unfold wp_low_to_high_prog', compilation_of; simpl; intros; cleanup.
+    unfold compilation_of in *; simpl in *; intros; cleanup.
+    split_ors; cleanup; eapply exec_deterministic_wrt_oracle in H0; eauto; cleanup.
+    invert_exec; intuition eauto.
+  Qed.
+
+  Lemma wp_high_to_low_ret :
+    forall T (v: T),
+    wp_high_to_low_prog' _ _ _ _ refinement _ (Ret v).
+  Proof.
+    unfold wp_high_to_low_prog', compilation_of; simpl; intros; cleanup.
+    unfold compilation_of in *; simpl; intros; cleanup.
+    split_ors; cleanup.
+    repeat invert_exec.
+    clear H4; eapply exec_to_wp; simpl; eauto.
+    econstructor.
+  Qed.
+
+  Lemma wcp_low_to_high_ret :
+    forall T (v: T),
+    wcp_low_to_high_prog' _ _ _ _ refinement _ (Ret v).
+  Proof.
+    unfold wcp_low_to_high_prog', compilation_of; simpl; intros; cleanup.
+    unfold compilation_of in *; simpl in *; intros; cleanup.
+    split_ors; cleanup; eapply exec_deterministic_wrt_oracle in H0; eauto; cleanup.
+    eexists; intuition eauto.
+    invert_exec; eauto.
+  Qed.
+
+  Lemma wcp_high_to_low_ret :
+    forall T (v: T),
+    wcp_high_to_low_prog' _ _ _ _ refinement _ (Ret v).
+  Proof.
+    unfold wcp_high_to_low_prog', compilation_of; simpl; intros; cleanup.
+    unfold compilation_of in *; simpl in *; intros; cleanup.
+    split_ors; cleanup.
+    repeat invert_exec.
+    eapply exec_to_wcp; eauto.
+    econstructor; eauto.
+  Qed.
+    
+  Theorem sbs_read :
+    forall a,
+      StrongBisimulationForProgram refinement (|Read a|).              
+  Proof.
+    intros.
+    eapply bisimulation_from_wp_prog; eauto.
+    exact exec_preserves_refinement.
+    exact exec_compiled_preserves_refinement.
+    eapply Build_WP_Bisimulation_prog.
+    apply wp_low_to_high_read.
+    apply wp_high_to_low_read.    
+    apply wcp_low_to_high_read.
+    apply wcp_high_to_low_read.
+  Qed.
+
+  Theorem sbs_write :
+    forall a lv,
+      StrongBisimulationForProgram refinement (|Write a lv|).              
+  Proof.
+    intros.
+    eapply bisimulation_from_wp_prog; eauto.
+    exact exec_preserves_refinement.
+    exact exec_compiled_preserves_refinement.
+    eapply Build_WP_Bisimulation_prog.
+    apply wp_low_to_high_write.
+    apply wp_high_to_low_write.
+    apply wcp_low_to_high_write.
+    apply wcp_high_to_low_write.
+  Qed.
+
+  Theorem sbs_start :
+      StrongBisimulationForProgram refinement (|Start|).              
+  Proof.
+    intros.
+    eapply bisimulation_from_wp_prog; eauto.
+    exact exec_preserves_refinement.
+    exact exec_compiled_preserves_refinement.
+    apply Build_WP_Bisimulation_prog.
+    apply wp_low_to_high_start.
+    apply wp_high_to_low_start.
+    apply wcp_low_to_high_start.
+    apply wcp_high_to_low_start.
+  Qed.
+
+  Theorem sbs_abort :
+      StrongBisimulationForProgram refinement (|Abort|).              
+  Proof.
+    intros.
+    eapply bisimulation_from_wp_prog; eauto.
+    exact exec_preserves_refinement.
+    exact exec_compiled_preserves_refinement.
+    apply Build_WP_Bisimulation_prog.
+    apply wp_low_to_high_abort.
+    apply wp_high_to_low_abort.
+    apply wcp_low_to_high_abort.
+    apply wcp_high_to_low_abort.
+  Qed.
+
+  Theorem sbs_commit :
+      StrongBisimulationForProgram refinement (|Commit|).              
+  Proof.
+    intros.
+    eapply bisimulation_from_wp_prog; eauto.
+    exact exec_preserves_refinement.
+    exact exec_compiled_preserves_refinement.
+    apply Build_WP_Bisimulation_prog.
+    apply wp_low_to_high_commit.
+    apply wp_high_to_low_commit.
+    apply wcp_low_to_high_commit.
+    apply wcp_high_to_low_commit.
+  Qed.
+
+  
+  Theorem sbs_ret :
+    forall T (v: T),
+    StrongBisimulationForProgram refinement (Ret v).              
+  Proof.
+    intros.
+    eapply bisimulation_from_wp_prog; eauto.
+    exact exec_preserves_refinement.
+    exact exec_compiled_preserves_refinement.
+    eapply Build_WP_Bisimulation_prog.
+    apply wp_low_to_high_ret.
+    apply wp_high_to_low_ret.
+    apply wcp_low_to_high_ret.
+    apply wcp_high_to_low_ret.
+  Qed.
+
+  Theorem sbs_bind:
+    forall T1 T2 (p1: high.(prog) T1) (p2: T1 -> high.(prog) T2),
+      StrongBisimulationForProgram refinement p1 ->
+      (forall t, StrongBisimulationForProgram refinement (p2 t)) ->
+      StrongBisimulationForProgram refinement (Bind p1 p2).
+  Proof.
+    intros.
+    edestruct H.
+    constructor; intros.
+    simpl in *; unfold compilation_of in *;
+    simpl in *; cleanup.
+
+    split; intros.
+    - (* Low to High *)
+      invert_exec; cleanup.
+      
+      + split_ors; cleanup.
+        eapply_fresh exec_deterministic_wrt_oracle_prefix in H5; eauto; cleanup.
+     
+        eapply_fresh exec_finished_deterministic_prefix in H5; eauto; cleanup.
+        eapply_fresh exec_deterministic_wrt_oracle in H6; eauto; cleanup.
+        edestruct strong_bisimulation_for_program_correct; eauto.
+        edestruct H2; eauto; simpl in *; cleanup; try intuition; clear H2 H3.
+        edestruct H0.
+        simpl in *; unfold compilation_of in *;
+        edestruct strong_bisimulation_for_program_correct0; eauto.
+        edestruct H2; eauto; simpl in *; cleanup; try intuition; clear H2 H3.
+        cleanup.
+        eexists; intuition eauto.
+        econstructor; eauto.
+        simpl; eauto.
+        
+      +
+        split_ors; cleanup;
+        split_ors; cleanup;
+        eapply_fresh exec_deterministic_wrt_oracle_prefix in H4; eauto; cleanup;
+        try solve [eapply_fresh exec_deterministic_wrt_oracle_prefix in H5; eauto; cleanup].
+        *
+          edestruct strong_bisimulation_for_program_correct; eauto.
+          edestruct H6; eauto; simpl in *; cleanup; try intuition; clear H6 H7.
+          exists (Crashed s); repeat (split; eauto).
+          eapply ExecBindCrash; eauto.
+
+        *
+          eapply_fresh exec_finished_deterministic_prefix in H5; eauto; cleanup.
+           eapply_fresh exec_deterministic_wrt_oracle in H6; eauto; cleanup.
+           edestruct strong_bisimulation_for_program_correct; eauto.
+           edestruct H2; eauto; simpl in *; cleanup; try intuition; clear H2 H3.
+           edestruct H0.
+           simpl in *; unfold compilation_of in *;
+           edestruct strong_bisimulation_for_program_correct0; eauto.
+           edestruct H2; eauto; simpl in *; cleanup; try intuition; clear H2 H3.
+           cleanup.
+           eexists; intuition eauto.
+           econstructor; eauto.
+           simpl; eauto.
+
+    - (* High to Low *)
+      invert_exec; cleanup.
+      
+
+      + split_ors; cleanup.
+        edestruct strong_bisimulation_for_program_correct; eauto.
+        edestruct H7; eauto; simpl in *; cleanup; try intuition; clear H7 H8.
+        eapply_fresh exec_deterministic_wrt_oracle_prefix in H2; eauto; cleanup.
+
+        edestruct strong_bisimulation_for_program_correct; eauto.
+        edestruct H9; eauto; simpl in *; cleanup; try intuition; clear H9 H10.
+        eapply_fresh exec_finished_deterministic_prefix in H2; eauto; cleanup.
+        simpl in *.
+        edestruct H0.
+        simpl in *; unfold compilation_of in *;
+        edestruct strong_bisimulation_for_program_correct0; eauto.
+        edestruct H4; eauto; simpl in *; cleanup; try intuition; clear H4 H9; cleanup.           
+        eapply_fresh exec_deterministic_wrt_oracle in H3; eauto; cleanup.
+        eexists; intuition eauto.
+        econstructor; eauto.
+        
+      +
+        split_ors; cleanup;
+        split_ors; cleanup;
+        eapply_fresh exec_deterministic_wrt_oracle_prefix in H4; eauto; cleanup;
+        try solve [eapply_fresh exec_deterministic_wrt_oracle_prefix in H5; eauto; cleanup].
+        *
+          edestruct strong_bisimulation_for_program_correct; eauto.
+          edestruct H6; eauto; simpl in *; cleanup; try intuition; clear H6 H7.
+          eapply_fresh exec_deterministic_wrt_oracle_prefix in H3; eauto; cleanup.
+          simpl in *.
+          exists (Crashed x5); repeat (split; eauto).
+          eapply ExecBindCrash; eauto.
+
+        *
+          edestruct strong_bisimulation_for_program_correct; eauto.
+          edestruct H8; eauto; simpl in *; cleanup; try intuition; clear H8 H9.
+          eapply_fresh exec_deterministic_wrt_oracle_prefix in H3; eauto; cleanup.
+
+        *
+          edestruct strong_bisimulation_for_program_correct; eauto.
+          edestruct H7; eauto; simpl in *; cleanup; try intuition; clear H7 H8.
+          eapply_fresh exec_deterministic_wrt_oracle_prefix in H3; eauto; cleanup.
+
+        *
+          edestruct strong_bisimulation_for_program_correct; eauto.
+          edestruct H9; eauto; simpl in *; cleanup; try intuition; clear H9 H10.
+           eapply_fresh exec_finished_deterministic_prefix in H3; eauto; cleanup.
+           edestruct H0.
+           simpl in *; unfold compilation_of in *;
+           edestruct strong_bisimulation_for_program_correct0; eauto.
+           edestruct H2; eauto; simpl in *; cleanup; try intuition; clear H2 H9.
+           cleanup.
+           eapply_fresh exec_deterministic_wrt_oracle in H4; eauto; cleanup.
+           eexists; intuition eauto.
+           econstructor; eauto.
+    Unshelve.
+    all: eauto.
+  Qed.
+
+  Hint Resolve sbs_read sbs_write sbs_start sbs_abort sbs_commit sbs_ret sbs_bind : core.
+  
+  Theorem sbs :
+      StrongBisimulation refinement.              
+  Proof.
+    apply bisimulation_restrict_prog.
+    induction p; eauto.
+    destruct p; eauto.
+  Qed.
+
+  Hint Resolve sbs : core.
+
+  Theorem sbs_general:
+    forall valid_state_h valid_prog_h,
+      exec_compiled_preserves_validity refinement
+        (refines_to_valid refinement valid_state_h) ->
+      
+      exec_preserves_validity TransactionalDiskLang valid_state_h ->
+      
+      StrongBisimulationForValidStates refinement
+        (refines_to_valid refinement valid_state_h)
+        valid_state_h
+        (compiles_to_valid refinement valid_prog_h)        
+        valid_prog_h.  
+  Proof.
+    intros.
+    eapply bisimulation_restrict_state; eauto.
+  Qed.
+
+End TransactionalDiskBisimulation.
+
+Section TransferToTransactionCache.
+
+   Lemma write_all_app :
+          forall V l1 l2 (l3 l4: list V) m,
+            length l1 = length l3 ->
+            (forall i, In i l1 -> m i <> None) ->
+            write_all m (l1++l2) (l3++l4) = write_all (write_all m l1 l3) l2 l4.
+        Proof.
+          induction l1; simpl in *; destruct l3; simpl in *;
+          intros; cleanup; try congruence.
+          destruct_fresh (m a); simpl in *.
+          erewrite IHl1; eauto.
+          intros; simpl.
+          unfold upd_disk.
+          destruct (addr_dec a i); subst; [rewrite upd_eq; eauto | rewrite upd_ne; eauto];
+          congruence.
+          exfalso; eapply H0; eauto.
+        Qed.
+      
+      Lemma write_all_merge_apply_list:
+        forall x6 x4 x,
+          refines_to (Some x6, x4) x ->
+          write_all x4 (map fst (rev x6)) (map snd (rev x6)) =
+          merge (apply_list empty_mem (rev x6)) x4.
+      Proof.
+        induction x6; simpl in *; intros; eauto.
+        unfold refines_to in *; simpl in *; cleanup.
+        repeat rewrite map_app; simpl in *.
+        rewrite write_all_app, apply_list_app in *; eauto; simpl in *.
+        unfold addrs_match in *.
+        destruct a, x; simpl in *.
+        erewrite IHx6; eauto.
+        unfold upd_disk.
+        extensionality a'; simpl.
+        unfold merge at 4; simpl.
+        - destruct (addr_dec a a'); subst; simpl;
+        [rewrite upd_eq; eauto
+        | rewrite upd_ne; eauto].
+          
+          + destruct_fresh (d0 a');
+            [| exfalso; eapply H1; eauto;
+               rewrite upd_eq; eauto; congruence ].
+            destruct_fresh (apply_list empty_mem (rev x6) a').
+            * edestruct merge_some_l
+                with (m2:= d0); eauto.
+              congruence.
+              cleanup.
+              pose proof H.
+              unfold merge in H; simpl.
+              rewrite D0, D in H.
+              destruct (merge (apply_list
+                 empty_mem (rev x6)) d0 a');
+              try congruence; cleanup.
+              rewrite upd_eq; eauto.
+      Admitted.
+              
+Lemma high_oracle_exists_ok':
+  forall T p2 p1 ol sl sl',
+    (exists sh, refines_to sl sh) ->
+    low.(exec) ol sl p1 sl' ->
+    compilation_of T p1 p2 ->
+    exists oh, oracle_refines_to T sl p2 ol oh.
+Proof.
+  unfold compilation_of;
+  induction p2; simpl; intros; cleanup.
+  - (* Start *)
+    destruct sl'.
+    {
+      eapply exec_to_sp with (P := fun o s => refines_to s x /\ o = ol /\ s = sl) in H0 as Hx; eauto.
+      simpl in *; cleanup.
+      eexists; left; do 2 eexists; intuition eauto.
+      destruct s; simpl in *.
+      unfold refines_to in *; simpl in *; intuition subst; eauto.
+    }
+    {
+      eapply exec_to_scp with (P := fun o s => refines_to s x /\ o = ol /\ s = sl) in H0 as Hx; eauto.
+      simpl in *; cleanup.
+       split_ors; cleanup; repeat (simpl in *; try split_ors; cleanup);
+       try (inversion H1; clear H1); cleanup; eauto;
+       try solve [
+             eexists; right; do 2 eexists; intuition eauto;
+             destruct s; simpl in *; cleanup; eauto ].
+    }
+  - (* Read *)
+    destruct sl'.
+    {
+      eapply exec_to_sp with (P := fun o s => refines_to s x /\ o = ol /\ s = sl) in H0 as Hx; eauto.
+      unfold read in Hx; simpl in Hx; cleanup;
+      cleanup; simpl in *; cleanup;
+      
+      eexists; left; do 2 eexists; intuition eauto;
+      destruct s; cleanup; simpl in *; cleanup; eauto.
+    }
+    {
+      eapply exec_to_scp with (P := fun o s => refines_to s x /\ o = ol /\ s = sl) in H0 as Hx; eauto.
+       unfold read in Hx; repeat (simpl in *; cleanup).
+       split_ors; cleanup; repeat (simpl in *; try split_ors; cleanup);
+       try (inversion H1; clear H1); cleanup; eauto;
+       try solve [
+             eexists; right; do 2 eexists; intuition eauto;
+             destruct s; simpl in *; cleanup; eauto ].
+       eexists; right; do 2 eexists; intuition eauto;
+             destruct s; simpl in *; cleanup; eauto.       
+    }
+  - (* Write *)
+    destruct sl'.
+    {
+      eapply exec_to_sp with (P := fun o s => refines_to s x /\ o = ol /\ s = sl) in H0 as Hx; eauto.
+      unfold write in Hx; simpl in *; cleanup;
+      cleanup; simpl in *; cleanup;      
+      try destruct s; cleanup; simpl in *; cleanup; eauto;
+      eexists; left; do 2 eexists; intuition eauto;
+      try destruct s; cleanup; simpl in *; cleanup; eauto.
+    }
+    {
+      eapply exec_to_scp with (P := fun o s => refines_to s x /\ o = ol /\ s = sl) in H0 as Hx; eauto.
+      unfold write in Hx; repeat (simpl in *; cleanup).
+       split_ors; cleanup; repeat (simpl in *; try split_ors; cleanup);
+       inversion H1; clear H1; cleanup; eauto;
+       try solve [
+             eexists; right; do 2 eexists; intuition eauto;
+             destruct s; simpl in *; cleanup; eauto ].
+       eexists; right; do 2 eexists; intuition eauto;
+       destruct s; simpl in *; cleanup; eauto.
+    }
+  - (* Commit *)
+    destruct sl'.
+    {
+      eapply exec_to_sp with (P := fun o s => refines_to s x /\ o = ol /\ s = sl) in H0 as Hx; eauto.
+      simpl in *; cleanup.
+      cleanup; simpl in *; cleanup;
+      eexists; left; do 2 eexists; intuition eauto;
+      destruct s; cleanup; simpl in *; cleanup; eauto.
+      eexists; intuition eauto.
+      rewrite <- map_fst_split, <- map_snd_split.
+      erewrite write_all_merge_apply_list; eauto.
+    }
+    {
+      eapply exec_to_scp with (P := fun o s => refines_to s x /\ o = ol /\ s = sl) in H0 as Hx; eauto.
+       simpl in *; cleanup.
+       split_ors; cleanup; repeat (simpl in *; try split_ors; cleanup);
+       try solve [
+             inversion H1; clear H1; cleanup; eauto;
+             eexists; right; do 2 eexists; intuition eauto;
+             destruct s; simpl in *; cleanup; eauto ].
+       
+       destruct s; simpl in *; cleanup; eauto.
+       eexists; right; do 2 eexists; intuition eauto.
+       admit. (* TODO: Solve this *)
+
+       inversion H1; clear H1; cleanup; eauto.
+       eexists; right; do 2 eexists; intuition eauto;
+       destruct s; simpl in *; cleanup; eauto.
+       admit. (* TODO: Solve this *)
+    
+       eexists; right; do 2 eexists; intuition eauto;
+       destruct s; simpl in *; cleanup; eauto.
+       right; intuition eauto; eexists; intuition eauto.
+       admit. (* TODO: Solve this *)       
+    }
+    
+  - (* Abort *)
+    destruct sl'.
+    {
+      eapply exec_to_sp with (P := fun o s => refines_to s x /\ o = ol /\ s = sl) in H0 as Hx; eauto.
+      simpl in *; cleanup.
+      eexists; left; do 2 eexists; intuition eauto.
+    }
+    {
+      eapply exec_to_scp with (P := fun o s => refines_to s x /\ o = ol /\ s = sl) in H0 as Hx; eauto.
+      simpl in *; cleanup.
+       split_ors; cleanup; repeat (simpl in *; try split_ors; cleanup);
+       try (inversion H1; clear H1); cleanup; eauto;
+       try solve [
+             eexists; right; do 2 eexists; intuition eauto;
+             destruct s; simpl in *; cleanup; eauto ].
+    }
+  - destruct sl'; eexists; eauto.
+  - (* Bind *)
+    invert_exec.
+    + (* Finished *)
+      edestruct IHp2; eauto.
+      eapply_fresh exec_compiled_preserves_refinement in H1; simpl in *;  eauto.
+      cleanup; simpl in *; eauto.
+      edestruct H; eauto.
+      do 5 eexists; repeat (split; eauto).
+      right; eauto.
+      do 3 eexists; repeat (split; eauto).        
+      unfold compilation_of; eauto.
+    + (* Crashed *)
+      split_ors; cleanup.
+      * (* p1 crashed *)
+        edestruct IHp2; eauto.
+        do 5 eexists; repeat (split; eauto).
+      * (* p2 Crashed *)
+        edestruct IHp2; eauto.
+        eapply_fresh exec_compiled_preserves_refinement in H1; simpl in *; eauto.
+        cleanup; simpl in *; eauto.
+        edestruct H; eauto.
+        do 5 eexists; repeat (split; eauto).
+        right; eauto.
+        do 3 eexists; repeat (split; eauto).
+        unfold compilation_of; eauto.
+        Unshelve.
+        all: constructor.
+Admitted.
+
+Lemma high_oracle_exists_ok :
+  high_oracle_exists refinement. 
+Proof.
+  unfold high_oracle_exists; intros.
+  eapply high_oracle_exists_ok'; eauto.
+Qed.
+
+
+Theorem transfer_to_TransactionCache:
+    forall related_states_h
+    valid_state_h
+    valid_prog_h,
+    
+    SelfSimulation
+      high
+      valid_state_h
+      valid_prog_h
+      related_states_h ->
+    
+    oracle_refines_to_same_from_related refinement related_states_h ->
+
+    exec_compiled_preserves_validity refinement                           
+    (refines_to_valid refinement valid_state_h) ->
+    
+    SelfSimulation
+      low
+      (refines_to_valid refinement valid_state_h)
+      (compiles_to_valid refinement valid_prog_h)
+      (refines_to_related refinement related_states_h).
+Proof.
+  intros; eapply transfer_high_to_low; eauto.
+  apply sbs.
+  apply high_oracle_exists_ok.
+Qed.
+
+End TransferToTransactionCache.
