src/Refinements/LogCacheToLoggedDisk/Definitions.v
@@ -1,0 +1,43 @@
+Require Import Framework CachedDiskLayer LoggedDiskLayer LogCache.
+Close Scope pred_scope.
+Import ListNotations.
+
+Local Definition low_op := CachedDiskOperation.
+Local Definition high_op := LoggedDiskOperation.
+Local Definition low := CachedDiskLang.
+Local Definition high := LoggedDiskLang.
+
+Definition compile_op T (p2: Operation.prog high_op T) : prog low T.
+ destruct p2.
+ exact (read a).
+ exact (write l l0).
+Defined.
+
+Definition oracle_refines_to_op T (d1: state low) (p: Operation.prog high_op T) o1 o2 : Prop :=
+   match p with
+     | Read a =>
+       (exists d1',
+          exec low o1 d1 (read a) (Crashed d1') /\
+          o2 = [CrashBefore]) \/
+       (exists d1' r,
+          exec low o1 d1 (read a) (Finished d1' r) /\
+          o2 = [Cont])
+         
+     | Write la lv =>
+       (exists d1',
+          exec low o1 d1 (write la lv) (Crashed d1') /\
+          ((d1' = d1 /\
+           o2 = [CrashBefore]) \/
+           (d1' <> d1 /\
+            o2 = [CrashAfter]))) \/
+       (exists d1' r,
+          exec low o1 d1 (write la lv) (Finished d1' r) /\          
+          o2 = [Cont] /\
+       (forall s ,(exists F, cached_log_rep F s d1) -> (exists F, cached_log_rep F (write_all s la lv) d1')))
+   end.
+
+  Definition refines_to (d1: state low) (d2: state high) :=
+    exists F, cached_log_rep F d2 d1.
+
+  Definition LoggedDiskOperationRefinement := Build_OperationRefinement compile_op refines_to oracle_refines_to_op.
+  Definition LoggedDiskRefinement := LiftRefinement LoggedDiskLang LoggedDiskOperationRefinement.
