src/Refinements/LogCacheToLoggedDisk/Refinement.v
@@ -1,0 +1,658 @@
+Require Import Framework FSParameters CachedDiskLayer.
+Require Import LogCache LoggedDiskLayer LogCacheToLoggedDisk.Definitions.
+Require Import ClassicalFacts FunctionalExtensionality Omega.
+
+Set Nested Proofs Allowed.
+
+Notation "'low'" := CachedDiskLang.
+Notation "'high'" := LoggedDiskLang.
+Notation "'refinement'" := LoggedDiskRefinement.
+
+Axiom excluded_middle_dec: forall P: Prop, {P}+{~P}.
+
+Section LoggedDiskBisimulation.
+
+  Lemma sp_impl:
+    forall T (p: prog low T) (P P': 
+     list (Language.token' CachedDiskOperation) -> Operation.state CachedDiskOperation -> Prop) s' t,
+      (forall o s, P' o s -> P o s) ->
+      strongest_postcondition low p P' t s' ->
+      strongest_postcondition low p P t s'.
+  Proof.
+    intros.
+    eapply sp_to_exec in H0; cleanup.
+    eapply exec_to_sp; eauto.
+  Qed.
+
+  Lemma sp_bind:
+    forall T T' (p1: prog low T) (p2: T -> prog low T') P s' t,
+      strongest_postcondition low (Bind p1 p2) P t s' ->
+      exists s0 t0,
+        strongest_postcondition low p1 (fun o s => exists o2, P (o++o2) s) t0 s0 /\
+        strongest_postcondition low (p2 t0)
+        (fun o s => strongest_postcondition low p1 (fun ox sx => P (ox++o) sx) t0 s0) t s'.
+  Proof.
+    intros.
+    eapply sp_to_exec in H; cleanup.
+    invert_exec.
+    do 2 eexists; split.
+    eapply exec_to_sp; eauto.
+    intros.            
+    repeat (eapply exec_to_sp; eauto).
+  Qed.
+
+
+  
+  Lemma exec_compiled_preserves_refinement:
+    exec_compiled_preserves_refinement refinement.
+  Proof.
+    unfold exec_compiled_preserves_refinement.
+    induction p2; simpl in *; intros; cleanup.
+    {
+      destruct p; simpl in *.
+      {
+        destruct ret.
+        eapply exec_to_sp with (P := fun o s => refines_to s x /\ s = s1) in H0; unfold refines_to in *; eauto.
+        simpl in *; repeat (cleanup; simpl in *); eauto.
+
+      eapply exec_to_scp with (P := fun o s => refines_to s x /\ s = s1) in H0; unfold refines_to in *; eauto.
+      simpl in *; repeat (try split_ors; cleanup; simpl in *); eauto;
+      inversion H0; cleanup; eauto.
+    }
+    {
+      destruct ret.
+          
+      assume (A:(forall s' t, strongest_postcondition CachedDiskLang (write l l0) (fun o s => exists s2, refines_to s s2) t s' ->
+                         exists s2' : state', refines_to s' s2')).
+
+      eapply A.
+      eapply exec_to_sp; eauto.
+
+      assume (A:(forall s', strongest_crash_postcondition CachedDiskLang (write l l0) (fun o s => exists s2, refines_to s s2) s' ->
+                         exists s2' : state', refines_to s' s2')).
+      eapply A.
+      eapply exec_to_scp; eauto.
+    }
+    }
+
+    {
+      destruct ret.
+      eapply exec_to_sp with (P := fun o s => refines_to s x /\ s = s1) in H0; unfold refines_to in *; eauto.
+      simpl in *; cleanup; simpl; eauto.
+      eapply exec_to_scp with (P := fun o s => refines_to s x /\ s = s1) in H0; unfold refines_to in *; eauto.
+      simpl in *; cleanup; simpl; eauto.
+    }
+
+    {
+      invert_exec; eauto.
+      split_ors; cleanup; eauto.
+      eapply IHp2 in H1; eauto.
+    }
+  Admitted.
+  
+  Lemma exec_preserves_refinement:
+    exec_preserves_refinement refinement.
+  Proof.
+    unfold exec_preserves_refinement; induction p; simpl; intros.
+    destruct ret.
+    {
+      eapply exec_to_sp with (P := fun o s => exists x, refines_to x s) in H0; eauto.
+      destruct p; simpl in *; cleanup; eauto.
+      clear H; unfold refines_to in *; cleanup.
+      admit. (* Doable *)
+    }
+    {
+      eapply exec_to_scp with (P := fun o s => exists x, refines_to x s) in H0; eauto.
+      destruct p; simpl in *; cleanup; eauto.
+      split_ors; cleanup; eauto.
+      clear H; unfold refines_to in *; cleanup.
+      admit. (* Doable *)
+    }
+
+    destruct ret.
+    {
+      eapply exec_to_sp with (P := fun o s => exists x, refines_to x s) in H0; eauto.
+      simpl in *; cleanup; eauto.
+    }
+    {
+      eapply exec_to_scp with (P := fun o s => exists x, refines_to x s) in H0; eauto.
+    }
+    
+    invert_exec.
+    eapply IHp in H1; eauto; simpl in *.
+    split_ors; cleanup; eauto.
+    eapply IHp in H1; eauto; simpl in *.
+  Admitted.
+      
+  Lemma merge_some_l:
+    forall AT AEQ V (m1: @mem AT AEQ V) m2 a v,
+      m1 a = Some v ->
+      m2 a <> None ->
+      exists vs, merge m1 m2 a = Some vs /\
+            fst vs = v.
+  Proof.
+    unfold merge; simpl; intros.
+    cleanup.
+    destruct (m2 a); try congruence; eauto.
+  Qed.
+  
+  Lemma merge_some_r:
+    forall AT AEQ V (m1: @mem AT AEQ V) m2 a,
+      m1 a = None ->
+      merge m1 m2 a = m2 a.
+  Proof.
+    unfold merge; simpl; intros.
+    cleanup; eauto.
+  Qed.
+
+  
+  Lemma cached_log_rep_cache_read :
+    forall F s2 s1 a v,
+      cached_log_rep F s2 s1 ->
+      fst s1 (data_start + a) = Some v ->
+      Disk.read s2 a = Some v.
+  Proof.
+    unfold cached_log_rep, Disk.read; intros.
+    cleanup; unfold shift; simpl in *.
+    eapply merge_some_l in H0; eauto; cleanup.
+    rewrite H0; eauto.
+    eapply H1.
+    congruence.
+  Qed.
+  
+  Lemma cached_log_rep_disk_read :
+    forall F s2 s1 a,
+      cached_log_rep F s2 s1 ->
+      fst s1 (data_start + a) = None ->
+      Disk.read s2 a = Disk.read (snd (snd s1)) (data_start + a).
+  Proof.
+    unfold cached_log_rep, Disk.read; intros.
+    unfold shift in *; simpl; cleanup.
+    erewrite merge_some_r; eauto.
+  Qed.
+
+  Lemma wp_low_to_high_read :
+    forall a,
+    wp_low_to_high_prog' _ _ _ _ LoggedDiskRefinement _ (|Read a|).
+  Proof.
+    unfold wp_low_to_high_prog', refines_to; simpl; intros; cleanup.
+    unfold refines_to in *; simpl; intros; cleanup.
+    split_ors; cleanup; eapply exec_deterministic_wrt_oracle in H0; eauto; cleanup.
+    eexists; intuition eauto.
+    eapply exec_to_sp with (P := fun o s => refines_to s s2 /\ s = s1) in H2; unfold refines_to in *; eauto.
+    simpl in *.
+    cleanup.
+    {        
+      cleanup; simpl in *; cleanup; eauto;
+      eexists; intuition eauto.
+      simpl in *.
+      eapply cached_log_rep_cache_read; eauto.
+      erewrite cached_log_rep_disk_read; eauto.
+      unfold Disk.read in *; simpl; cleanup; eauto.
+    }
+
+    cleanup; simpl in *.
+    {
+      cleanup.
+      eexists; split; eauto; simpl in *.
+      unfold refines_to in *; cleanup.
+      erewrite cached_log_rep_disk_read; eauto.
+      unfold Disk.read in *; simpl; cleanup; eauto.
+      split_ors; cleanup.
+      eapply exec_deterministic_wrt_oracle in H1; eauto; cleanup.
+      eexists; intuition eauto.
+      
+    }
+    {
+      cleanup; eauto.
+      eexists; intuition eauto.
+      erewrite cached_log_rep_disk_read; eauto.      
+      unfold Disk.read in *; simpl; cleanup; eauto.
+    }
+  Qed.
+
+  Lemma wp_high_to_low_read :
+    forall a,
+    wp_high_to_low_prog' _ _ _ _ LoggedDiskRefinement _ (|Read a|).
+  Proof.
+    unfold wp_high_to_low_prog', , refines_to; simpl; intros; cleanup.
+    unfold , refines_to in *; simpl; intros; cleanup.
+    split_ors; cleanup.
+    repeat invert_exec.
+    eapply exec_to_wp; eauto.
+
+    eapply exec_to_sp with (P := fun o s => refines_to s s2' /\ s = s1) in H0; unfold refines_to in *; eauto.
+
+    unfold read in *; simpl in *.
+    cleanup; simpl in *.
+    destruct x4; simpl in *; cleanup; eauto.
+    - destruct x2; simpl in *; split; eauto.
+      eapply cached_log_rep_cache_read in H0; eauto; cleanup.
+      congruence.
+      
+    - destruct x2, s0; simpl in *; split; eauto.
+      eapply cached_log_rep_disk_read in H0; eauto; cleanup.
+      unfold Disk.read in *; simpl in *; cleanup; eauto.
+      simpl in *; congruence.
+  Qed.
+
+
+  Lemma wcp_low_to_high_read :
+    forall a,
+    wcp_low_to_high_prog' _ _ _ _ LoggedDiskRefinement _ (|Read a|).
+  Proof.
+    unfold wcp_low_to_high_prog', , refines_to; simpl; intros; cleanup.
+    unfold  in *; simpl in *; intros; cleanup.
+    split_ors; cleanup; eapply exec_deterministic_wrt_oracle in H0; eauto; cleanup.
+    eexists; intuition eauto.
+    destruct x0, s0.
+    eapply exec_to_scp with (P := fun o s => refines_to s s2) in H3; unfold refines_to in *; eauto.
+    simpl in *; cleanup.
+    repeat (split_ors; repeat (cleanup; simpl in *);
+    try solve [ inversion H; cleanup; eexists; eauto ]).
+  Qed.
+
+  Lemma wcp_high_to_low_read :
+    forall a,
+    wcp_high_to_low_prog' _ _ _ _ LoggedDiskRefinement _ (|Read a|).
+  Proof.
+    unfold wcp_high_to_low_prog', , refines_to; simpl; intros; cleanup.
+    unfold , refines_to in *; simpl in *; intros; cleanup.
+    split_ors; cleanup.
+    repeat invert_exec.
+    eapply exec_to_wcp; eauto.
+    destruct x1, s1.
+    eapply exec_to_scp with (P := fun o s => refines_to s s2') in H0; unfold refines_to in *; eauto.
+    simpl in *; cleanup.
+    repeat (split_ors; repeat (cleanup; simpl in *);
+    try solve [ inversion H0; cleanup; eexists; eauto ]).
+  Qed.
+
+  Lemma wp_low_to_high_write :
+    forall a vl,
+    wp_low_to_high_prog' _ _ _ _ LoggedDiskRefinement _ (|Write a vl|).
+  Proof.
+    unfold wp_low_to_high_prog', , refines_to; simpl; intros; cleanup.
+    unfold , refines_to in *; simpl in *; intros; cleanup.
+    split_ors; cleanup; eapply exec_deterministic_wrt_oracle in H0; eauto; cleanup.
+    eapply exec_to_sp with (P := fun o s => refines_to s s2) in H3; unfold refines_to in *; eauto.
+    unfold write in *.
+    simpl in *; cleanup.
+    eexists; intuition eauto.
+  Qed.
+
+  Lemma wp_high_to_low_write :
+    forall a vl,
+    wp_high_to_low_prog' _ _ _ _ LoggedDiskRefinement _ (|Write a vl|).
+  Proof.
+    unfold wp_high_to_low_prog', , refines_to; simpl; intros; cleanup.
+    unfold , refines_to in *; simpl; intros; cleanup.
+    repeat invert_exec.
+    repeat (split_ors; cleanup).
+    eapply exec_to_wp; eauto.
+    eexists; eauto.
+    destruct x3; eauto.
+  Qed.
+
+  
+  Lemma wcp_low_to_high_write :
+    forall a vl,
+    wcp_low_to_high_prog' _ _ _ _ LoggedDiskRefinement _ (|Write a vl|).
+  Proof.
+    unfold wcp_low_to_high_prog', , refines_to; simpl; intros; cleanup.
+    unfold , refines_to in *; simpl; intros; cleanup.
+    split_ors; cleanup; eapply exec_deterministic_wrt_oracle in H0; eauto; cleanup.
+    split_ors; cleanup;
+    eexists; intuition eauto.
+    right; intuition eauto.
+    eapply exec_to_scp with (P := fun o s => refines_to s s2 /\ s = s1) in H3.
+    2: unfold refines_to; eauto.
+    admit. (* TODO: Check this *)
+  Admitted.
+
+  Lemma wcp_high_to_low_write :
+    forall a vl,
+    wcp_high_to_low_prog' _ _ _ _ LoggedDiskRefinement _ (|Write a vl|).
+  Proof.
+    unfold wcp_high_to_low_prog', , refines_to; simpl; intros; cleanup.
+    unfold , refines_to in *; simpl; intros; cleanup.
+    repeat split_ors; cleanup; repeat invert_exec;
+    eapply exec_to_wcp; eauto;
+    split_ors; cleanup; eauto.
+    admit. (* TODO: Check this *)
+  Admitted.
+
+
+  Lemma wp_low_to_high_ret :
+    forall T (v: T),
+    wp_low_to_high_prog' _ _ _ _ LoggedDiskRefinement _ (Ret v).
+  Proof.
+    unfold wp_low_to_high_prog', , refines_to; simpl; intros; cleanup.
+    unfold , refines_to in *; simpl in *; intros; cleanup.
+    split_ors; cleanup; eapply exec_deterministic_wrt_oracle in H0; eauto; cleanup.
+    invert_exec; intuition eauto.
+  Qed.
+
+  Lemma wp_high_to_low_ret :
+    forall T (v: T),
+    wp_high_to_low_prog' _ _ _ _ LoggedDiskRefinement _ (Ret v).
+  Proof.
+    unfold wp_high_to_low_prog', , refines_to; simpl; intros; cleanup.
+    unfold , refines_to in *; simpl; intros; cleanup.
+    split_ors; cleanup.
+    repeat invert_exec.
+    eapply exec_to_wp; eauto.
+    econstructor; eauto.
+  Qed.
+
+  Lemma wcp_low_to_high_ret :
+    forall T (v: T),
+    wcp_low_to_high_prog' _ _ _ _ LoggedDiskRefinement _ (Ret v).
+  Proof.
+    unfold wcp_low_to_high_prog', , refines_to; simpl; intros; cleanup.
+    unfold , refines_to in *; simpl in *; intros; cleanup.
+    split_ors; cleanup; eapply exec_deterministic_wrt_oracle in H0; eauto; cleanup.
+    eexists; intuition eauto.
+    invert_exec; eauto.
+  Qed.
+
+  Lemma wcp_high_to_low_ret :
+    forall T (v: T),
+    wcp_high_to_low_prog' _ _ _ _ LoggedDiskRefinement _ (Ret v).
+  Proof.
+    unfold wcp_high_to_low_prog', , refines_to; simpl; intros; cleanup.
+    unfold , refines_to in *; simpl in *; intros; cleanup.
+    split_ors; cleanup.
+    repeat invert_exec.
+    eapply exec_to_wcp; eauto.
+    econstructor; eauto.
+  Qed.
+    
+  Theorem sbs_read :
+    forall a,
+      StrongBisimulationForProgram LoggedDiskRefinement (|Read a|).              
+  Proof.
+    intros.
+    eapply bisimulation_from_wp_prog; eauto.
+    exact exec_preserves_refinement.
+    exact exec_compiled_preserves_refinement.
+    eapply Build_WP_Bisimulation_prog.
+    apply wp_low_to_high_read.
+    apply wp_high_to_low_read.    
+    apply wcp_low_to_high_read.
+    apply wcp_high_to_low_read.
+  Qed.
+
+  Theorem sbs_write :
+    forall a lv,
+      StrongBisimulationForProgram LoggedDiskRefinement (|Write a lv|).              
+  Proof.
+    intros.
+    eapply bisimulation_from_wp_prog; eauto.
+    exact exec_preserves_refinement.
+    exact exec_compiled_preserves_refinement.
+    eapply Build_WP_Bisimulation_prog.
+    apply wp_low_to_high_write.
+    apply wp_high_to_low_write.
+    apply wcp_low_to_high_write.
+    apply wcp_high_to_low_write.
+  Qed.
+
+  
+  Theorem sbs_ret :
+    forall T (v: T),
+    StrongBisimulationForProgram LoggedDiskRefinement
+      (Ret v).              
+  Proof.
+    intros.
+    eapply bisimulation_from_wp_prog; eauto.
+    exact exec_preserves_refinement.
+    exact exec_compiled_preserves_refinement.
+    eapply Build_WP_Bisimulation_prog.
+    apply wp_low_to_high_ret.
+    apply wp_high_to_low_ret.
+    apply wcp_low_to_high_ret.
+    apply wcp_high_to_low_ret.
+  Qed.
+
+  Theorem sbs_bind:
+    forall T1 T2 (p1: high.(prog) T1) (p2: T1 -> high.(prog) T2),
+      StrongBisimulationForProgram LoggedDiskRefinement p1 ->
+      (forall t, StrongBisimulationForProgram LoggedDiskRefinement (p2 t)) ->
+      StrongBisimulationForProgram LoggedDiskRefinement (Bind p1 p2).
+  Proof.
+    intros.
+    edestruct H.
+    constructor; intros.
+    simpl in *; unfold  in *;
+    simpl in *; cleanup.
+
+    split; intros.
+    - (* Low to High *)
+      invert_exec; cleanup.
+      
+      + split_ors; cleanup.
+        eapply_fresh exec_deterministic_wrt_oracle_prefix in H5; eauto; cleanup.
+     
+        eapply_fresh exec_finished_deterministic_prefix in H5; eauto; cleanup.
+        eapply_fresh exec_deterministic_wrt_oracle in H6; eauto; cleanup.
+        edestruct strong_bisimulation_for_program_correct; eauto.
+        edestruct H2; eauto; simpl in *; cleanup; try intuition; clear H2 H3.
+        edestruct H0.
+        simpl in *; unfold  in *;
+        edestruct strong_bisimulation_for_program_correct0; eauto.
+        edestruct H2; eauto; simpl in *; cleanup; try intuition; clear H2 H3.
+        cleanup.
+        eexists; intuition eauto.
+        econstructor; eauto.
+        simpl; eauto.
+        
+      +
+        split_ors; cleanup;
+        split_ors; cleanup;
+        eapply_fresh exec_deterministic_wrt_oracle_prefix in H4; eauto; cleanup;
+        try solve [eapply_fresh exec_deterministic_wrt_oracle_prefix in H5; eauto; cleanup].
+        *
+          edestruct strong_bisimulation_for_program_correct; eauto.
+          edestruct H6; eauto; simpl in *; cleanup; try intuition; clear H6 H7.
+          exists (Crashed s); repeat (split; eauto).
+          eapply ExecBindCrash; eauto.
+
+        *
+          eapply_fresh exec_finished_deterministic_prefix in H5; eauto; cleanup.
+           eapply_fresh exec_deterministic_wrt_oracle in H6; eauto; cleanup.
+           edestruct strong_bisimulation_for_program_correct; eauto.
+           edestruct H2; eauto; simpl in *; cleanup; try intuition; clear H2 H3.
+           edestruct H0.
+           simpl in *; unfold  in *;
+           edestruct strong_bisimulation_for_program_correct0; eauto.
+           edestruct H2; eauto; simpl in *; cleanup; try intuition; clear H2 H3.
+           cleanup.
+           eexists; intuition eauto.
+           econstructor; eauto.
+           simpl; eauto.
+
+    - (* High to Low *)
+      invert_exec; cleanup.
+      
+
+      + split_ors; cleanup.
+        edestruct strong_bisimulation_for_program_correct; eauto.
+        edestruct H7; eauto; simpl in *; cleanup; try intuition; clear H7 H8.
+        eapply_fresh exec_deterministic_wrt_oracle_prefix in H2; eauto; cleanup.
+
+        edestruct strong_bisimulation_for_program_correct; eauto.
+        edestruct H9; eauto; simpl in *; cleanup; try intuition; clear H9 H10.
+        eapply_fresh exec_finished_deterministic_prefix in H2; eauto; cleanup.
+        simpl in *.
+        edestruct H0.
+        simpl in *; unfold  in *;
+        edestruct strong_bisimulation_for_program_correct0; eauto.
+        edestruct H4; eauto; simpl in *; cleanup; try intuition; clear H4 H9; cleanup.           
+        eapply_fresh exec_deterministic_wrt_oracle in H3; eauto; cleanup.
+        eexists; intuition eauto.
+        econstructor; eauto.
+        
+      +
+        split_ors; cleanup;
+        split_ors; cleanup;
+        eapply_fresh exec_deterministic_wrt_oracle_prefix in H4; eauto; cleanup;
+        try solve [eapply_fresh exec_deterministic_wrt_oracle_prefix in H5; eauto; cleanup].
+        *
+          edestruct strong_bisimulation_for_program_correct; eauto.
+          edestruct H6; eauto; simpl in *; cleanup; try intuition; clear H6 H7.
+          eapply_fresh exec_deterministic_wrt_oracle_prefix in H3; eauto; cleanup.
+          simpl in *.
+          exists (Crashed x5); repeat (split; eauto).
+          eapply ExecBindCrash; eauto.
+
+        *
+          edestruct strong_bisimulation_for_program_correct; eauto.
+          edestruct H8; eauto; simpl in *; cleanup; try intuition; clear H8 H9.
+          eapply_fresh exec_deterministic_wrt_oracle_prefix in H3; eauto; cleanup.
+
+        *
+          edestruct strong_bisimulation_for_program_correct; eauto.
+          edestruct H7; eauto; simpl in *; cleanup; try intuition; clear H7 H8.
+          eapply_fresh exec_deterministic_wrt_oracle_prefix in H3; eauto; cleanup.
+
+        *
+          edestruct strong_bisimulation_for_program_correct; eauto.
+          edestruct H9; eauto; simpl in *; cleanup; try intuition; clear H9 H10.
+           eapply_fresh exec_finished_deterministic_prefix in H3; eauto; cleanup.
+           edestruct H0.
+           simpl in *; unfold  in *;
+           edestruct strong_bisimulation_for_program_correct0; eauto.
+           edestruct H2; eauto; simpl in *; cleanup; try intuition; clear H2 H9.
+           cleanup.
+           eapply_fresh exec_deterministic_wrt_oracle in H4; eauto; cleanup.
+           eexists; intuition eauto.
+           econstructor; eauto.
+    Unshelve.
+    all: eauto.
+  Qed.
+
+  Hint Resolve sbs_read sbs_ret sbs_write sbs_bind : core.
+  
+  Theorem sbs :
+      StrongBisimulation LoggedDiskRefinement.              
+  Proof.
+    apply bisimulation_restrict_prog.
+    induction p; eauto.
+    destruct p; eauto.
+  Qed.
+
+  Hint Resolve sbs : core.
+
+  Theorem sbs_general:
+    forall valid_state_h valid_prog_h,
+      exec_compiled_preserves_validity LoggedDiskRefinement
+        (refines_to_valid LoggedDiskRefinement valid_state_h) ->
+      
+      exec_preserves_validity LoggedDiskLang valid_state_h ->
+      
+      StrongBisimulationForValidStates LoggedDiskRefinement
+        (refines_to_valid LoggedDiskRefinement valid_state_h)
+        valid_state_h
+        (compiles_to_valid LoggedDiskRefinement valid_prog_h)        
+        valid_prog_h.  
+  Proof.
+    intros.
+    eapply bisimulation_restrict_state; eauto.
+  Qed.
+End LoggedDiskBisimulation.
+
+Section TransferToCachedDisk.
+              
+Lemma high_oracle_exists_ok':
+  forall T p2 p1 ol sl sl',
+    (exists sh, refines_to sl sh) ->
+    low.(exec) ol sl p1 sl' ->
+     T p1 p2 ->
+    exists oh, oracle_refines_to T sl p2 ol oh.
+Proof.
+  unfold refines_to, ;
+  induction p2; simpl; intros; cleanup.
+  {
+    destruct p; simpl in *.
+    - (* Read *)
+      destruct sl'; do 2 eexists; intuition eauto.
+    - (* Write *)
+      destruct sl'; try solve [do 2 eexists; intuition eauto].
+      do 2 eexists; intuition eauto;
+      right; eauto.
+      eapply exec_to_sp with (P := fun o s => refines_to s x /\ o = ol /\ s = sl) in H0 as Hx; unfold refines_to in *; eauto.
+      do 2 eexists; intuition eauto.
+      admit. (* Doable *)
+      
+    destruct (excluded_middle_dec (s = sl));
+    do 2 eexists; intuition eauto;
+    left; eauto.
+  }  
+  - (* Ret *)
+    destruct sl'; eexists; eauto.
+  - (* Bind *)
+    invert_exec.
+    + (* Finished *)
+      edestruct IHp2; eauto.
+      eapply_fresh exec_compiled_preserves_refinement in H1; simpl in *; unfold refines_to in *; eauto.
+      cleanup; simpl in *; eauto.
+      edestruct H; eauto.
+      do 5 eexists; repeat (split; eauto).
+      right; eauto.
+      do 3 eexists; repeat (split; eauto).        
+      unfold ; eauto.
+    + (* Crashed *)
+      split_ors; cleanup.
+      * (* p1 crashed *)
+        edestruct IHp2; eauto.
+        do 5 eexists; repeat (split; eauto).
+      * (* p2 Crashed *)
+        edestruct IHp2; eauto.
+        eapply_fresh exec_compiled_preserves_refinement in H1; simpl in *; unfold refines_to in *; eauto.
+        cleanup; simpl in *; eauto.
+        edestruct H; eauto.
+        do 5 eexists; repeat (split; eauto).
+        right; eauto.
+        do 3 eexists; repeat (split; eauto).
+        unfold ; eauto.
+        Unshelve.
+        eauto.
+Admitted.
+
+Lemma high_oracle_exists_ok :
+  high_oracle_exists LoggedDiskRefinement. 
+Proof.
+  unfold high_oracle_exists; intros.
+  eapply high_oracle_exists_ok'; eauto.
+Qed.
+
+
+Theorem transfer_to_CachedDisk:
+    forall related_states_h
+    valid_state_h
+    valid_prog_h,
+    
+    SelfSimulation
+      LoggedDiskLang
+      valid_state_h
+      valid_prog_h
+      related_states_h ->
+    
+    oracle_refines_to_same_from_related LoggedDiskRefinement related_states_h ->
+
+    exec_compiled_preserves_validity LoggedDiskRefinement                           
+    (refines_to_valid LoggedDiskRefinement valid_state_h) ->
+    
+    SelfSimulation
+      CachedDiskLang
+      (refines_to_valid LoggedDiskRefinement valid_state_h)
+      (compiles_to_valid LoggedDiskRefinement valid_prog_h)
+      (refines_to_related LoggedDiskRefinement related_states_h).
+Proof.
+  intros; eapply transfer_high_to_low; eauto.
+  apply sbs.
+  apply high_oracle_exists_ok.
+Qed.
+
+End TransferToCachedDisk.
