src/Refinements/TransactionToTransactionalDisk/Definitions.v
@@ -1,0 +1,118 @@
+Require Import Framework FSParameters.
+Require Import TransactionCacheLayer TransactionalDiskLayer Transaction.
+Close Scope pred_scope.
+Import ListNotations.
+
+Local Definition low_op := TransactionCacheOperation.
+Local Definition high_op := (TransactionalDiskOperation data_length).
+Local Definition low := TransactionCacheLang.
+Local Definition high := (TransactionalDiskLang data_length).
+
+Fixpoint apply_list {A AEQ V} (m: @mem A AEQ V) l :=
+  match l with
+  | nil =>
+    m
+  | av :: l' =>
+    apply_list (upd m (fst av) (snd av)) l'
+  end.
+
+Definition compile  T (p2: Operation.prog high_op T) : prog low T.
+  destruct p2.
+  exact start.
+  exact (read a).
+  exact (write a v).
+  exact commit.
+  exact abort.
+Defined.
+
+Definition oracle_refines_to T (d1: state low) (p: Operation.prog high_op T) o1 o2 : Prop :=
+     match p with
+     | Start =>
+       (exists d1' r,
+          exec low o1 d1 start (Finished d1' r) /\
+          o2 = [Cont] /\
+          d1' = (Some [], snd d1)) \/
+       
+       (exists d1',
+          exec low o1 d1 start (Crashed d1') /\
+          ((o2 = [CrashBefore] /\
+            d1' = d1) \/
+           
+           (o2 = [CrashAfter] /\
+            d1' = (Some [], snd d1))))
+         
+     | Read a =>
+       (exists d1' r,
+          exec low o1 d1 (read a) (Finished d1' r) /\
+          o2 = [Cont] /\
+          d1' = d1) \/
+       
+       (exists d1',
+          exec low o1 d1 (read a) (Crashed d1') /\
+          (o2 = [CrashBefore] \/
+          (o2 = [CrashAfter] /\
+           exists l, fst d1 = Some l /\
+           exists v, get_latest l a = Some v \/ (get_latest l a = None /\ Disk.read (snd d1) a = Some v))) /\
+          d1' = d1)
+         
+     | Write a v =>
+       (exists d1' r,
+          exec low o1 d1 (write a v) (Finished d1' r) /\          
+          ((o2 = [Cont] /\
+           d1' = (option_map (fun l => (a, v)::l) (fst d1), snd d1)) \/
+          (o2 = [TxnFull] /\
+           d1' = d1)
+          )
+       ) \/
+       
+       (exists d1',
+          exec low o1 d1 (write a v) (Crashed d1') /\
+          ((o2 = [CrashBefore] /\
+            d1' = d1) \/
+           
+           (o2 = [CrashAfter] /\
+            fst d1 <> None /\
+            d1' = (option_map (fun l => (a, v)::l) (fst d1), snd d1))))
+
+     | Commit =>
+       (exists d1' r,
+          exec low o1 d1 commit (Finished d1' r) /\
+          o2 = [Cont] /\
+          (exists l, fst d1 = Some l /\
+                d1' = (None, merge (apply_list empty_mem (rev l)) (snd d1)))) \/
+       
+       (exists d1',
+          exec low o1 d1 commit (Crashed d1') /\
+          ((o2 =[CrashBefore] /\
+           d1' = d1) \/
+           (o2 = [CrashAfter] /\
+            (exists l, fst d1 = Some l /\
+                d1' = (None,  merge (apply_list empty_mem (rev l)) (snd d1) )))))
+         
+     | Abort =>
+       (exists d1' r,
+          exec low o1 d1 abort (Finished d1' r) /\
+          o2 = [Cont]) \/
+       
+       (exists d1',
+          exec low o1 d1 abort (Crashed d1') /\
+          ((o2 = [CrashBefore] /\
+           d1' = d1) \/
+           (o2 = [CrashAfter] /\
+          d1' = (None, snd d1))))
+     end.
+
+   Definition refines_to (d1: state low) (d2: state high) :=     
+     match fst d1 with
+     | Some l =>
+       let txn_cache := apply_list empty_mem (rev l) in
+       fst d2 = txn_cache /\
+       addrs_match txn_cache (snd d1)
+     | None =>
+       fst d2 = empty_mem
+     end /\
+     snd d2 = snd d1.
+
+   
+  Definition TransactionalDiskOperationRefinement := Build_OperationRefinement compile refines_to oracle_refines_to.
+  Definition TransactionalDiskRefinement := LiftRefinement high TransactionalDiskOperationRefinement.
