src/Refinements/TransactionToTransactionalDisk/TransactionalDiskRefinement.v
@@ -1,0 +1,1 @@
+Require Export TransactionToTransactionalDisk.Definitions TransactionToTransactionalDisk.Refinement.
